proofs/fstar/extraction/Polytune.Faand.fst
@@ -6,8 +6,12 @@ open FStar.Mul
 let _ =
   (* This module has implicit dependencies, here we make them explicit. *)
   (* The implicit dependencies arise from typeclasses instances. *)
-  let open Hax_lib.Prop in
   let open Polytune.Channel in
+  let open Rand.Distributions.Distribution in
+  let open Rand.Distributions.Other in
+  let open Rand.Rng in
+  let open Rand_chacha.Chacha in
+  let open Rand_core in
   let open Serde.De in
   let open Serde.De.Impls in
   let open Serde.Ser in
@@ -36,122 +40,88 @@ type t_Error =
   | Error_InvalidHashLength : t_Error
   | Error_OtErr : Polytune.Swankyot.t_Error -> t_Error
 
-/// Represents a cryptographic commitment as a fixed-size 32-byte array (a BLAKE3 hash).
-type t_Commitment = | Commitment : t_Array u8 (mk_usize 32) -> t_Commitment
-
-/// Represents a triple of commitments, needed for the fashare protocol.
-type t_CommitmentTriple =
-  | CommitmentTriple : t_Commitment -> t_Commitment -> t_Commitment -> t_CommitmentTriple
-
+/// Converts an `ot::Error` into a custom `Error` type.
 [@@ FStar.Tactics.Typeclasses.tcinstance]
+let impl_1: Core.Convert.t_From t_Error Polytune.Swankyot.t_Error =
+  {
+    f_from_pre = (fun (e: Polytune.Swankyot.t_Error) -> true);
+    f_from_post = (fun (e: Polytune.Swankyot.t_Error) (out: t_Error) -> true);
+    f_from = fun (e: Polytune.Swankyot.t_Error) -> Error_OtErr e <: t_Error
+  }
+
+/// Implements same broadcast with abort as broadcast, but only the first element of the tuple in
+/// the vector is broadcasted, the second element is simply sent to all parties.
 assume
-val impl_8': Core.Fmt.t_Debug t_CommitmentTriple
-
-let impl_8 = impl_8'
-
-[@@ FStar.Tactics.Typeclasses.tcinstance]
-assume
-val impl_9': Core.Clone.t_Clone t_CommitmentTriple
-
-let impl_9 = impl_9'
-
-[@@ FStar.Tactics.Typeclasses.tcinstance]
-assume
-val e_ee_2__impl': Serde.Ser.t_Serialize t_CommitmentTriple
-
-let e_ee_2__impl = e_ee_2__impl'
-
-[@@ FStar.Tactics.Typeclasses.tcinstance]
-assume
-val e_ee_3__impl': Serde.De.t_Deserialize t_CommitmentTriple
-
-let e_ee_3__impl = e_ee_3__impl'
-
-[@@ FStar.Tactics.Typeclasses.tcinstance]
-assume
-val impl_12': Core.Cmp.t_PartialEq t_CommitmentTriple t_CommitmentTriple
-
-let impl_12 = impl_12'
-
-/// Represents a vector of `u8` values.
-type t_VectorU8 = | VectorU8 : Alloc.Vec.t_Vec u8 Alloc.Alloc.t_Global -> t_VectorU8
-
-[@@ FStar.Tactics.Typeclasses.tcinstance]
-assume
-val impl_13': Core.Fmt.t_Debug t_VectorU8
-
-let impl_13 = impl_13'
-
-[@@ FStar.Tactics.Typeclasses.tcinstance]
-assume
-val impl_14': Core.Clone.t_Clone t_VectorU8
-
-let impl_14 = impl_14'
-
-[@@ FStar.Tactics.Typeclasses.tcinstance]
-assume
-val e_ee_4__impl': Serde.Ser.t_Serialize t_VectorU8
-
-let e_ee_4__impl = e_ee_4__impl'
-
-[@@ FStar.Tactics.Typeclasses.tcinstance]
-assume
-val e_ee_5__impl': Serde.De.t_Deserialize t_VectorU8
-
-let e_ee_5__impl = e_ee_5__impl'
-
-[@@ FStar.Tactics.Typeclasses.tcinstance]
-assume
-val impl_16': Core.Cmp.t_PartialEq t_VectorU8 t_VectorU8
-
-let impl_16 = impl_16'
-
-/// Commits to a value using the BLAKE3 cryptographic hash function.
-/// This is not a general-purpose commitment scheme, the input value is assumed to have high entropy.
-assume
-val commit': value: t_Slice u8 -> t_Commitment
-
-let commit = commit'
-
-/// Verifies if a given value matches a previously generated commitment.
-/// This is not a general-purpose commitment scheme, the input value is assumed to have high entropy.
-assume
-val open_commitment': commitment: t_Commitment -> value: t_Slice u8 -> bool
-
-let open_commitment = open_commitment'
-
-/// Implements broadcast with abort based on Goldwasser and Lindell\'s protocol
-/// for all parties at once, where each party sends its vector to all others.
-/// The function returns the vector received and verified by broadcast.
-assume
-val broadcast':
+val broadcast_first_send_second':
     #v_T: Type0 ->
+    #v_S: Type0 ->
     #iimpl_951670863_: Type0 ->
-    {| i2: Core.Clone.t_Clone v_T |} ->
-    {| i3: Serde.Ser.t_Serialize v_T |} ->
-    {| i4: Serde.De.t_DeserializeOwned v_T |} ->
-    {| i5: Core.Fmt.t_Debug v_T |} ->
-    {| i6: Core.Cmp.t_PartialEq v_T v_T |} ->
-    {| i7: Polytune.Channel.t_Channel iimpl_951670863_ |} ->
+    {| i3: Core.Clone.t_Clone v_T |} ->
+    {| i4: Serde.Ser.t_Serialize v_T |} ->
+    {| i5: Serde.De.t_DeserializeOwned v_T |} ->
+    {| i6: Core.Fmt.t_Debug v_T |} ->
+    {| i7: Core.Cmp.t_PartialEq v_T v_T |} ->
+    {| i8: Core.Clone.t_Clone v_S |} ->
+    {| i9: Serde.Ser.t_Serialize v_S |} ->
+    {| i10: Serde.De.t_DeserializeOwned v_S |} ->
+    {| i11: Core.Fmt.t_Debug v_S |} ->
+    {| i12: Core.Cmp.t_PartialEq v_S v_S |} ->
+    {| i13: Polytune.Channel.t_Channel iimpl_951670863_ |} ->
     channel: iimpl_951670863_ ->
     i: usize ->
     n: usize ->
     phase: string ->
-    vec: t_Slice v_T ->
+    vec: t_Slice (Alloc.Vec.t_Vec (v_T & v_S) Alloc.Alloc.t_Global) ->
     len: usize
   -> (iimpl_951670863_ &
       Core.Result.t_Result
-        (Alloc.Vec.t_Vec (Alloc.Vec.t_Vec v_T Alloc.Alloc.t_Global) Alloc.Alloc.t_Global) t_Error)
+        (Alloc.Vec.t_Vec (Alloc.Vec.t_Vec (v_T & v_S) Alloc.Alloc.t_Global) Alloc.Alloc.t_Global)
+        t_Error)
 
-let broadcast
-      (#v_T #iimpl_951670863_: Type0)
-      (#[FStar.Tactics.Typeclasses.tcresolve ()] i2: Core.Clone.t_Clone v_T)
-      (#[FStar.Tactics.Typeclasses.tcresolve ()] i3: Serde.Ser.t_Serialize v_T)
-      (#[FStar.Tactics.Typeclasses.tcresolve ()] i4: Serde.De.t_DeserializeOwned v_T)
-      (#[FStar.Tactics.Typeclasses.tcresolve ()] i5: Core.Fmt.t_Debug v_T)
-      (#[FStar.Tactics.Typeclasses.tcresolve ()] i6: Core.Cmp.t_PartialEq v_T v_T)
-      (#[FStar.Tactics.Typeclasses.tcresolve ()] i7: Polytune.Channel.t_Channel iimpl_951670863_)
-     = broadcast' #v_T #iimpl_951670863_ #i2 #i3 #i4 #i5 #i6 #i7
+unfold
+let broadcast_first_send_second
+      (#v_T #v_S #iimpl_951670863_: Type0)
+      (#[FStar.Tactics.Typeclasses.tcresolve ()] i3: Core.Clone.t_Clone v_T)
+      (#[FStar.Tactics.Typeclasses.tcresolve ()] i4: Serde.Ser.t_Serialize v_T)
+      (#[FStar.Tactics.Typeclasses.tcresolve ()] i5: Serde.De.t_DeserializeOwned v_T)
+      (#[FStar.Tactics.Typeclasses.tcresolve ()] i6: Core.Fmt.t_Debug v_T)
+      (#[FStar.Tactics.Typeclasses.tcresolve ()] i7: Core.Cmp.t_PartialEq v_T v_T)
+      (#[FStar.Tactics.Typeclasses.tcresolve ()] i8: Core.Clone.t_Clone v_S)
+      (#[FStar.Tactics.Typeclasses.tcresolve ()] i9: Serde.Ser.t_Serialize v_S)
+      (#[FStar.Tactics.Typeclasses.tcresolve ()] i10: Serde.De.t_DeserializeOwned v_S)
+      (#[FStar.Tactics.Typeclasses.tcresolve ()] i11: Core.Fmt.t_Debug v_S)
+      (#[FStar.Tactics.Typeclasses.tcresolve ()] i12: Core.Cmp.t_PartialEq v_S v_S)
+      (#[FStar.Tactics.Typeclasses.tcresolve ()] i13: Polytune.Channel.t_Channel iimpl_951670863_)
+     =
+  broadcast_first_send_second' #v_T #v_S #iimpl_951670863_ #i3 #i4 #i5 #i6 #i7 #i8 #i9 #i10 #i11
+    #i12 #i13
+
+/// Multi-party coin tossing to generate shared randomness in a secure, distributed manner.
+/// This function generates a shared random number generator (RNG) using multi-party
+/// coin tossing in a secure multi-party computation (MPC) setting. Each participant contributes
+/// to the randomness generation, and all contributions are combined securely to generate
+/// a final shared random seed. This shared seed is then used to create a `ChaCha20Rng`, a
+/// cryptographically secure random number generator.
+assume
+val shared_rng':
+    #iimpl_951670863_: Type0 ->
+    {| i1: Polytune.Channel.t_Channel iimpl_951670863_ |} ->
+    channel: iimpl_951670863_ ->
+    i: usize ->
+    n: usize
+  -> (iimpl_951670863_ & Core.Result.t_Result Rand_chacha.Chacha.t_ChaCha20Rng t_Error)
+
+unfold
+let shared_rng
+      (#iimpl_951670863_: Type0)
+      (#[FStar.Tactics.Typeclasses.tcresolve ()] i1: Polytune.Channel.t_Channel iimpl_951670863_)
+     = shared_rng' #iimpl_951670863_ #i1
+
+assume
+val zero_rng': Prims.unit -> Rand_chacha.Chacha.t_ChaCha20Rng
+
+unfold
+let zero_rng = zero_rng'
 
 /// Protocol PI_aBit^n that performs F_aBit^n from the paper
 /// [Global-Scale Secure Multiparty Computation](https://dl.acm.org/doi/pdf/10.1145/3133956.3133979).
@@ -162,355 +132,820 @@ let broadcast
 /// each pair of parties and then checking the validity of the MACs and keys by checking the XOR
 /// of a linear combination of the bits, keys and the MACs and then removing 2 * RHO objects,
 /// where RHO is the statistical security parameter.
-assume
-val fabitn':
-    #iimpl_951670863_: Type0 ->
-    {| i1: Polytune.Channel.t_Channel iimpl_951670863_ |} ->
-    channel: iimpl_951670863_ ->
-    delta: Polytune.Data_types.t_Delta ->
-    i: usize ->
-    n: usize ->
-    l: usize ->
-    shared_two_by_two: Alloc.Vec.t_Vec Rand_chacha.Chacha.t_ChaCha20Rng Alloc.Alloc.t_Global
-  -> Prims.Pure
-      (iimpl_951670863_ &
-        Core.Result.t_Result
-          (Alloc.Vec.t_Vec Polytune.Data_types.t_Share Alloc.Alloc.t_Global &
-            Rand_chacha.Chacha.t_ChaCha20Rng) t_Error)
-      (requires l <=. Core.Num.impl_usize__MAX)
-      (fun _ -> Prims.l_True)
-
 let fabitn
-      (#iimpl_951670863_: Type0)
-      (#[FStar.Tactics.Typeclasses.tcresolve ()] i1: Polytune.Channel.t_Channel iimpl_951670863_)
-     = fabitn' #iimpl_951670863_ #i1
-
-/// Protocol PI_aShare that performs F_aShare from the paper
-/// [Global-Scale Secure Multiparty Computation](https://dl.acm.org/doi/pdf/10.1145/3133956.3133979).
-/// This protocol allows parties to generate and distribute authenticated random shares securely.
-/// It consists of the following steps:
-/// 1. **Random Bit String Generation**: Each party picks a random bit string of a specified length.
-/// 2. **Autenticated Bit Generation**: The parties generate random authenticated bit shares.
-/// 3. **Commitment and Verification**:
-///    - The parties compute commitments based on a subset of their shares and broadcast these to ensure consistency.
-///    - They then verify these commitments by performing decommitments and checking the validity of the
-///      MACs against the commitments.
-/// 4. **Return Shares**: Finally, the function returns the first `l` authenticated bit shares.
-let fashare
       (#iimpl_951670863_: Type0)
       (#[FStar.Tactics.Typeclasses.tcresolve ()] i1: Polytune.Channel.t_Channel iimpl_951670863_)
       (channel: iimpl_951670863_)
       (delta: Polytune.Data_types.t_Delta)
       (i n l: usize)
       (shared_two_by_two: Alloc.Vec.t_Vec Rand_chacha.Chacha.t_ChaCha20Rng Alloc.Alloc.t_Global)
-    : Prims.Pure
-      (iimpl_951670863_ &
-        Core.Result.t_Result
-          (Alloc.Vec.t_Vec Polytune.Data_types.t_Share Alloc.Alloc.t_Global &
-            Rand_chacha.Chacha.t_ChaCha20Rng) t_Error)
-      (requires l <=. (Core.Num.impl_usize__MAX -! v_RHO <: usize))
-      (fun _ -> Prims.l_True) =
-  let tmp0, out:(iimpl_951670863_ &
-    Core.Result.t_Result
-      (Alloc.Vec.t_Vec Polytune.Data_types.t_Share Alloc.Alloc.t_Global &
-        Rand_chacha.Chacha.t_ChaCha20Rng) t_Error) =
-    fabitn #iimpl_951670863_ channel delta i n (l +! v_RHO <: usize) shared_two_by_two
+    : (iimpl_951670863_ &
+      Core.Result.t_Result
+        (Alloc.Vec.t_Vec Polytune.Data_types.t_Share Alloc.Alloc.t_Global &
+          Rand_chacha.Chacha.t_ChaCha20Rng) t_Error) =
+  let three_rho:usize = mk_usize 3 *! v_RHO in
+  let lprime:usize = l +! three_rho in
+  let (x: Alloc.Vec.t_Vec bool Alloc.Alloc.t_Global):Alloc.Vec.t_Vec bool Alloc.Alloc.t_Global =
+    Core.Iter.Traits.Iterator.f_collect #(Core.Iter.Adapters.Map.t_Map
+          (Core.Ops.Range.t_Range usize) (usize -> bool))
+      #FStar.Tactics.Typeclasses.solve
+      #(Alloc.Vec.t_Vec bool Alloc.Alloc.t_Global)
+      (Core.Iter.Traits.Iterator.f_map #(Core.Ops.Range.t_Range usize)
+          #FStar.Tactics.Typeclasses.solve
+          #bool
+          ({ Core.Ops.Range.f_start = mk_usize 0; Core.Ops.Range.f_end = lprime }
+            <:
+            Core.Ops.Range.t_Range usize)
+          (fun temp_0_ ->
+              let _:usize = temp_0_ in
+              Rand.random #bool () <: bool)
+        <:
+        Core.Iter.Adapters.Map.t_Map (Core.Ops.Range.t_Range usize) (usize -> bool))
   in
-  let channel:iimpl_951670863_ = tmp0 in
-  match
-    out
+  let keys:Alloc.Vec.t_Vec (Alloc.Vec.t_Vec u128 Alloc.Alloc.t_Global) Alloc.Alloc.t_Global =
+    Alloc.Vec.from_elem #(Alloc.Vec.t_Vec u128 Alloc.Alloc.t_Global)
+      (Alloc.Vec.from_elem #u128 (mk_u128 0) lprime <: Alloc.Vec.t_Vec u128 Alloc.Alloc.t_Global)
+      n
+  in
+  let macs:Alloc.Vec.t_Vec (Alloc.Vec.t_Vec u128 Alloc.Alloc.t_Global) Alloc.Alloc.t_Global =
+    Alloc.Vec.from_elem #(Alloc.Vec.t_Vec u128 Alloc.Alloc.t_Global)
+      (Alloc.Vec.from_elem #u128 (mk_u128 0) lprime <: Alloc.Vec.t_Vec u128 Alloc.Alloc.t_Global)
+      n
+  in
+  if
+    ~.((Alloc.Vec.impl_1__len #Rand_chacha.Chacha.t_ChaCha20Rng
+          #Alloc.Alloc.t_Global
+          shared_two_by_two
+        <:
+        usize) =.
+      n
+      <:
+      bool)
+  then
+    channel,
+    (Core.Result.Result_Err (Error_InvalidLength <: t_Error)
+      <:
+      Core.Result.t_Result
+        (Alloc.Vec.t_Vec Polytune.Data_types.t_Share Alloc.Alloc.t_Global &
+          Rand_chacha.Chacha.t_ChaCha20Rng) t_Error)
     <:
-    Core.Result.t_Result
-      (Alloc.Vec.t_Vec Polytune.Data_types.t_Share Alloc.Alloc.t_Global &
-        Rand_chacha.Chacha.t_ChaCha20Rng) t_Error
-  with
-  | Core.Result.Result_Ok (xishares, multi_shared_rand) ->
-    let d0:Alloc.Vec.t_Vec u128 Alloc.Alloc.t_Global =
-      Alloc.Vec.from_elem #u128 (mk_u128 0) v_RHO
-    in
-    let d1:Alloc.Vec.t_Vec u128 Alloc.Alloc.t_Global =
-      Alloc.Vec.from_elem #u128 (mk_u128 0) v_RHO
-    in
-    let c0_c1_cm:Alloc.Vec.t_Vec t_CommitmentTriple Alloc.Alloc.t_Global =
-      Alloc.Vec.impl__with_capacity #t_CommitmentTriple v_RHO
-    in
-    let (dmvec: Alloc.Vec.t_Vec t_VectorU8 Alloc.Alloc.t_Global):Alloc.Vec.t_Vec t_VectorU8
-      Alloc.Alloc.t_Global =
-      Alloc.Vec.impl__with_capacity #t_VectorU8 v_RHO
-    in
-    let lprime:usize = l +! v_RHO in
-    let c0_c1_cm, d0, d1, dmvec:(Alloc.Vec.t_Vec t_CommitmentTriple Alloc.Alloc.t_Global &
-      Alloc.Vec.t_Vec u128 Alloc.Alloc.t_Global &
-      Alloc.Vec.t_Vec u128 Alloc.Alloc.t_Global &
-      Alloc.Vec.t_Vec t_VectorU8 Alloc.Alloc.t_Global) =
-      Rust_primitives.Hax.Folds.fold_range (mk_usize 0)
-        v_RHO
+    (iimpl_951670863_ &
+      Core.Result.t_Result
+        (Alloc.Vec.t_Vec Polytune.Data_types.t_Share Alloc.Alloc.t_Global &
+          Rand_chacha.Chacha.t_ChaCha20Rng) t_Error)
+  else
+    match
+      Rust_primitives.Hax.Folds.fold_range_return (mk_usize 0)
+        n
         (fun temp_0_ temp_1_ ->
-            let c0_c1_cm, d0, d1, dmvec:(Alloc.Vec.t_Vec t_CommitmentTriple Alloc.Alloc.t_Global &
-              Alloc.Vec.t_Vec u128 Alloc.Alloc.t_Global &
-              Alloc.Vec.t_Vec u128 Alloc.Alloc.t_Global &
-              Alloc.Vec.t_Vec t_VectorU8 Alloc.Alloc.t_Global) =
+            let channel, keys, macs:(iimpl_951670863_ &
+              Alloc.Vec.t_Vec (Alloc.Vec.t_Vec u128 Alloc.Alloc.t_Global) Alloc.Alloc.t_Global &
+              Alloc.Vec.t_Vec (Alloc.Vec.t_Vec u128 Alloc.Alloc.t_Global) Alloc.Alloc.t_Global) =
               temp_0_
             in
             let _:usize = temp_1_ in
-            Hax_lib.Prop.impl_Prop__and #Hax_lib.Prop.t_Prop
-              (Core.Convert.f_into #bool
-                  #Hax_lib.Prop.t_Prop
-                  #FStar.Tactics.Typeclasses.solve
-                  ((Alloc.Vec.impl_1__len #Polytune.Data_types.t_Share
-                        #Alloc.Alloc.t_Global
-                        xishares
-                      <:
-                      usize) =.
-                    lprime
-                    <:
-                    bool)
-                <:
-                Hax_lib.Prop.t_Prop)
-              (Hax_lib.Prop.v_forall #usize
-                  #Hax_lib.Prop.t_Prop
-                  (fun ll ->
-                      let ll:usize = ll in
-                      Hax_lib.Prop.implies #bool
-                        #bool
-                        ((mk_usize 0 <=. ll <: bool) && (ll <. lprime <: bool) &&
-                          ((Alloc.Vec.impl_1__len #Polytune.Data_types.t_Share
-                                #Alloc.Alloc.t_Global
-                                xishares
-                              <:
-                              usize) =.
-                            lprime
-                            <:
-                            bool))
-                        ((Alloc.Vec.impl_1__len #(Polytune.Data_types.t_Mac &
-                                Polytune.Data_types.t_Key)
-                              #Alloc.Alloc.t_Global
-                              (xishares.[ ll ] <: Polytune.Data_types.t_Share)
-                                .Polytune.Data_types._1
-                                .Polytune.Data_types._0
-                            <:
-                            usize) =.
-                          n
-                          <:
-                          bool)
-                      <:
-                      Hax_lib.Prop.t_Prop)
-                <:
-                Hax_lib.Prop.t_Prop)
-            <:
-            Hax_lib.Prop.t_Prop)
-        (c0_c1_cm, d0, d1, dmvec
+            true)
+        (channel, keys, macs
           <:
-          (Alloc.Vec.t_Vec t_CommitmentTriple Alloc.Alloc.t_Global &
-            Alloc.Vec.t_Vec u128 Alloc.Alloc.t_Global &
-            Alloc.Vec.t_Vec u128 Alloc.Alloc.t_Global &
-            Alloc.Vec.t_Vec t_VectorU8 Alloc.Alloc.t_Global))
-        (fun temp_0_ r ->
-            let c0_c1_cm, d0, d1, dmvec:(Alloc.Vec.t_Vec t_CommitmentTriple Alloc.Alloc.t_Global &
-              Alloc.Vec.t_Vec u128 Alloc.Alloc.t_Global &
-              Alloc.Vec.t_Vec u128 Alloc.Alloc.t_Global &
-              Alloc.Vec.t_Vec t_VectorU8 Alloc.Alloc.t_Global) =
+          (iimpl_951670863_ &
+            Alloc.Vec.t_Vec (Alloc.Vec.t_Vec u128 Alloc.Alloc.t_Global) Alloc.Alloc.t_Global &
+            Alloc.Vec.t_Vec (Alloc.Vec.t_Vec u128 Alloc.Alloc.t_Global) Alloc.Alloc.t_Global))
+        (fun temp_0_ k ->
+            let channel, keys, macs:(iimpl_951670863_ &
+              Alloc.Vec.t_Vec (Alloc.Vec.t_Vec u128 Alloc.Alloc.t_Global) Alloc.Alloc.t_Global &
+              Alloc.Vec.t_Vec (Alloc.Vec.t_Vec u128 Alloc.Alloc.t_Global) Alloc.Alloc.t_Global) =
               temp_0_
             in
-            let r:usize = r in
-            let xishare:Polytune.Data_types.t_Share = xishares.[ l +! r <: usize ] in
-            let dm:Alloc.Vec.t_Vec u8 Alloc.Alloc.t_Global =
-              Alloc.Vec.impl__with_capacity #u8 (n *! mk_usize 16 <: usize)
-            in
-            let dm:Alloc.Vec.t_Vec u8 Alloc.Alloc.t_Global =
-              Alloc.Vec.impl_1__push #u8
-                #Alloc.Alloc.t_Global
-                dm
-                (cast (xishare.Polytune.Data_types._0 <: bool) <: u8)
-            in
-            let d0, dm:(Alloc.Vec.t_Vec u128 Alloc.Alloc.t_Global &
-              Alloc.Vec.t_Vec u8 Alloc.Alloc.t_Global) =
-              Rust_primitives.Hax.Folds.fold_range (mk_usize 0)
-                n
-                (fun temp_0_ temp_1_ ->
-                    let d0, dm:(Alloc.Vec.t_Vec u128 Alloc.Alloc.t_Global &
-                      Alloc.Vec.t_Vec u8 Alloc.Alloc.t_Global) =
-                      temp_0_
-                    in
-                    let _:usize = temp_1_ in
-                    true)
-                (d0, dm
+            let k:usize = k in
+            if k =. i <: bool
+            then
+              Core.Ops.Control_flow.ControlFlow_Continue
+              (channel, keys, macs
+                <:
+                (iimpl_951670863_ &
+                  Alloc.Vec.t_Vec (Alloc.Vec.t_Vec u128 Alloc.Alloc.t_Global) Alloc.Alloc.t_Global &
+                  Alloc.Vec.t_Vec (Alloc.Vec.t_Vec u128 Alloc.Alloc.t_Global) Alloc.Alloc.t_Global))
+              <:
+              Core.Ops.Control_flow.t_ControlFlow
+                (Core.Ops.Control_flow.t_ControlFlow
+                    (iimpl_951670863_ &
+                      Core.Result.t_Result
+                        (Alloc.Vec.t_Vec Polytune.Data_types.t_Share Alloc.Alloc.t_Global &
+                          Rand_chacha.Chacha.t_ChaCha20Rng) t_Error)
+                    (Prims.unit &
+                      (iimpl_951670863_ &
+                        Alloc.Vec.t_Vec (Alloc.Vec.t_Vec u128 Alloc.Alloc.t_Global)
+                          Alloc.Alloc.t_Global &
+                        Alloc.Vec.t_Vec (Alloc.Vec.t_Vec u128 Alloc.Alloc.t_Global)
+                          Alloc.Alloc.t_Global)))
+                (iimpl_951670863_ &
+                  Alloc.Vec.t_Vec (Alloc.Vec.t_Vec u128 Alloc.Alloc.t_Global) Alloc.Alloc.t_Global &
+                  Alloc.Vec.t_Vec (Alloc.Vec.t_Vec u128 Alloc.Alloc.t_Global) Alloc.Alloc.t_Global)
+            else
+              let shared:Rand_chacha.Chacha.t_ChaCha20Rng = shared_two_by_two.[ k ] in
+              let
+              (shared_rand: Alloc.Vec.t_Vec Rand_chacha.Chacha.t_ChaCha20Rng Alloc.Alloc.t_Global):Alloc.Vec.t_Vec
+                Rand_chacha.Chacha.t_ChaCha20Rng Alloc.Alloc.t_Global =
+                Alloc.Vec.from_elem #Rand_chacha.Chacha.t_ChaCha20Rng
+                  (zero_rng () <: Rand_chacha.Chacha.t_ChaCha20Rng)
+                  n
+              in
+              if i <. k
+              then
+                let tmp0, out:(iimpl_951670863_ &
+                  Core.Result.t_Result
+                    (Alloc.Vec.t_Vec u128 Alloc.Alloc.t_Global & Rand_chacha.Chacha.t_ChaCha20Rng)
+                    Polytune.Swankyot.t_Error) =
+                  Polytune.Ot.kos_ot_sender #iimpl_951670863_
+                    channel
+                    delta.Polytune.Data_types._0
+                    lprime
+                    k
+                    shared
+                in
+                let channel:iimpl_951670863_ = tmp0 in
+                match
+                  out
                   <:
-                  (Alloc.Vec.t_Vec u128 Alloc.Alloc.t_Global &
-                    Alloc.Vec.t_Vec u8 Alloc.Alloc.t_Global))
-                (fun temp_0_ k ->
-                    let d0, dm:(Alloc.Vec.t_Vec u128 Alloc.Alloc.t_Global &
-                      Alloc.Vec.t_Vec u8 Alloc.Alloc.t_Global) =
-                      temp_0_
-                    in
-                    let k:usize = k in
-                    if k =. i <: bool
-                    then
-                      d0, dm
-                      <:
-                      (Alloc.Vec.t_Vec u128 Alloc.Alloc.t_Global &
-                        Alloc.Vec.t_Vec u8 Alloc.Alloc.t_Global)
-                    else
-                      let mac, key:(Polytune.Data_types.t_Mac & Polytune.Data_types.t_Key) =
-                        xishare.Polytune.Data_types._1.Polytune.Data_types._0.[ k ]
-                      in
-                      let d0:Alloc.Vec.t_Vec u128 Alloc.Alloc.t_Global =
-                        Rust_primitives.Hax.Monomorphized_update_at.update_at_usize d0
-                          r
-                          (key.Polytune.Data_types._0 ^. (d0.[ r ] <: u128) <: u128)
-                      in
-                      let dm:Alloc.Vec.t_Vec u8 Alloc.Alloc.t_Global =
-                        Core.Iter.Traits.Collect.f_extend #(Alloc.Vec.t_Vec u8 Alloc.Alloc.t_Global)
-                          #u8
+                  Core.Result.t_Result
+                    (Alloc.Vec.t_Vec u128 Alloc.Alloc.t_Global & Rand_chacha.Chacha.t_ChaCha20Rng)
+                    Polytune.Swankyot.t_Error
+                with
+                | Core.Result.Result_Ok (lhs, lhs_1_) ->
+                  let keys:Alloc.Vec.t_Vec (Alloc.Vec.t_Vec u128 Alloc.Alloc.t_Global)
+                    Alloc.Alloc.t_Global =
+                    Rust_primitives.Hax.Monomorphized_update_at.update_at_usize keys k lhs
+                  in
+                  let shared_rand:Alloc.Vec.t_Vec Rand_chacha.Chacha.t_ChaCha20Rng
+                    Alloc.Alloc.t_Global =
+                    Rust_primitives.Hax.Monomorphized_update_at.update_at_usize shared_rand k lhs_1_
+                  in
+                  let _:Prims.unit = () in
+                  let tmp0, out:(iimpl_951670863_ &
+                    Core.Result.t_Result
+                      (Alloc.Vec.t_Vec u128 Alloc.Alloc.t_Global & Rand_chacha.Chacha.t_ChaCha20Rng)
+                      Polytune.Swankyot.t_Error) =
+                    Polytune.Ot.kos_ot_receiver #iimpl_951670863_
+                      channel
+                      (Core.Ops.Deref.f_deref #(Alloc.Vec.t_Vec bool Alloc.Alloc.t_Global)
                           #FStar.Tactics.Typeclasses.solve
-                          #(t_Array u8 (mk_usize 16))
-                          dm
-                          (Core.Num.impl_u128__to_be_bytes mac.Polytune.Data_types._0
-                            <:
-                            t_Array u8 (mk_usize 16))
-                      in
-                      d0, dm
+                          x
+                        <:
+                        t_Slice bool)
+                      k
+                      shared
+                  in
+                  let channel:iimpl_951670863_ = tmp0 in
+                  (match
+                      out
                       <:
-                      (Alloc.Vec.t_Vec u128 Alloc.Alloc.t_Global &
-                        Alloc.Vec.t_Vec u8 Alloc.Alloc.t_Global))
-            in
-            let d1:Alloc.Vec.t_Vec u128 Alloc.Alloc.t_Global =
-              Rust_primitives.Hax.Monomorphized_update_at.update_at_usize d1
-                r
-                ((d0.[ r ] <: u128) ^. delta.Polytune.Data_types._0 <: u128)
-            in
-            let c0:t_Commitment =
-              commit (Core.Num.impl_u128__to_be_bytes (d0.[ r ] <: u128) <: t_Slice u8)
-            in
-            let c1:t_Commitment =
-              commit (Core.Num.impl_u128__to_be_bytes (d1.[ r ] <: u128) <: t_Slice u8)
-            in
-            let cm:t_Commitment =
-              commit (Core.Ops.Deref.f_deref #(Alloc.Vec.t_Vec u8 Alloc.Alloc.t_Global)
-                    #FStar.Tactics.Typeclasses.solve
-                    dm
+                      Core.Result.t_Result
+                        (Alloc.Vec.t_Vec u128 Alloc.Alloc.t_Global &
+                          Rand_chacha.Chacha.t_ChaCha20Rng) Polytune.Swankyot.t_Error
+                    with
+                    | Core.Result.Result_Ok (lhs, lhs_2_) ->
+                      let macs:Alloc.Vec.t_Vec (Alloc.Vec.t_Vec u128 Alloc.Alloc.t_Global)
+                        Alloc.Alloc.t_Global =
+                        Rust_primitives.Hax.Monomorphized_update_at.update_at_usize macs k lhs
+                      in
+                      let shared_rand:Alloc.Vec.t_Vec Rand_chacha.Chacha.t_ChaCha20Rng
+                        Alloc.Alloc.t_Global =
+                        Rust_primitives.Hax.Monomorphized_update_at.update_at_usize shared_rand
+                          k
+                          lhs_2_
+                      in
+                      let _:Prims.unit = () in
+                      Core.Ops.Control_flow.ControlFlow_Continue
+                      (channel, keys, macs
+                        <:
+                        (iimpl_951670863_ &
+                          Alloc.Vec.t_Vec (Alloc.Vec.t_Vec u128 Alloc.Alloc.t_Global)
+                            Alloc.Alloc.t_Global &
+                          Alloc.Vec.t_Vec (Alloc.Vec.t_Vec u128 Alloc.Alloc.t_Global)
+                            Alloc.Alloc.t_Global))
+                      <:
+                      Core.Ops.Control_flow.t_ControlFlow
+                        (Core.Ops.Control_flow.t_ControlFlow
+                            (iimpl_951670863_ &
+                              Core.Result.t_Result
+                                (Alloc.Vec.t_Vec Polytune.Data_types.t_Share Alloc.Alloc.t_Global &
+                                  Rand_chacha.Chacha.t_ChaCha20Rng) t_Error)
+                            (Prims.unit &
+                              (iimpl_951670863_ &
+                                Alloc.Vec.t_Vec (Alloc.Vec.t_Vec u128 Alloc.Alloc.t_Global)
+                                  Alloc.Alloc.t_Global &
+                                Alloc.Vec.t_Vec (Alloc.Vec.t_Vec u128 Alloc.Alloc.t_Global)
+                                  Alloc.Alloc.t_Global)))
+                        (iimpl_951670863_ &
+                          Alloc.Vec.t_Vec (Alloc.Vec.t_Vec u128 Alloc.Alloc.t_Global)
+                            Alloc.Alloc.t_Global &
+                          Alloc.Vec.t_Vec (Alloc.Vec.t_Vec u128 Alloc.Alloc.t_Global)
+                            Alloc.Alloc.t_Global)
+                    | Core.Result.Result_Err err ->
+                      Core.Ops.Control_flow.ControlFlow_Break
+                      (Core.Ops.Control_flow.ControlFlow_Break
+                        (channel,
+                          (Core.Result.Result_Err
+                            (Core.Convert.f_from #t_Error
+                                #Polytune.Swankyot.t_Error
+                                #FStar.Tactics.Typeclasses.solve
+                                err)
+                            <:
+                            Core.Result.t_Result
+                              (Alloc.Vec.t_Vec Polytune.Data_types.t_Share Alloc.Alloc.t_Global &
+                                Rand_chacha.Chacha.t_ChaCha20Rng) t_Error)
+                          <:
+                          (iimpl_951670863_ &
+                            Core.Result.t_Result
+                              (Alloc.Vec.t_Vec Polytune.Data_types.t_Share Alloc.Alloc.t_Global &
+                                Rand_chacha.Chacha.t_ChaCha20Rng) t_Error))
+                        <:
+                        Core.Ops.Control_flow.t_ControlFlow
+                          (iimpl_951670863_ &
+                            Core.Result.t_Result
+                              (Alloc.Vec.t_Vec Polytune.Data_types.t_Share Alloc.Alloc.t_Global &
+                                Rand_chacha.Chacha.t_ChaCha20Rng) t_Error)
+                          (Prims.unit &
+                            (iimpl_951670863_ &
+                              Alloc.Vec.t_Vec (Alloc.Vec.t_Vec u128 Alloc.Alloc.t_Global)
+                                Alloc.Alloc.t_Global &
+                              Alloc.Vec.t_Vec (Alloc.Vec.t_Vec u128 Alloc.Alloc.t_Global)
+                                Alloc.Alloc.t_Global)))
+                      <:
+                      Core.Ops.Control_flow.t_ControlFlow
+                        (Core.Ops.Control_flow.t_ControlFlow
+                            (iimpl_951670863_ &
+                              Core.Result.t_Result
+                                (Alloc.Vec.t_Vec Polytune.Data_types.t_Share Alloc.Alloc.t_Global &
+                                  Rand_chacha.Chacha.t_ChaCha20Rng) t_Error)
+                            (Prims.unit &
+                              (iimpl_951670863_ &
+                                Alloc.Vec.t_Vec (Alloc.Vec.t_Vec u128 Alloc.Alloc.t_Global)
+                                  Alloc.Alloc.t_Global &
+                                Alloc.Vec.t_Vec (Alloc.Vec.t_Vec u128 Alloc.Alloc.t_Global)
+                                  Alloc.Alloc.t_Global)))
+                        (iimpl_951670863_ &
+                          Alloc.Vec.t_Vec (Alloc.Vec.t_Vec u128 Alloc.Alloc.t_Global)
+                            Alloc.Alloc.t_Global &
+                          Alloc.Vec.t_Vec (Alloc.Vec.t_Vec u128 Alloc.Alloc.t_Global)
+                            Alloc.Alloc.t_Global))
+                | Core.Result.Result_Err err ->
+                  Core.Ops.Control_flow.ControlFlow_Break
+                  (Core.Ops.Control_flow.ControlFlow_Break
+                    (channel,
+                      (Core.Result.Result_Err
+                        (Core.Convert.f_from #t_Error
+                            #Polytune.Swankyot.t_Error
+                            #FStar.Tactics.Typeclasses.solve
+                            err)
+                        <:
+                        Core.Result.t_Result
+                          (Alloc.Vec.t_Vec Polytune.Data_types.t_Share Alloc.Alloc.t_Global &
+                            Rand_chacha.Chacha.t_ChaCha20Rng) t_Error)
+                      <:
+                      (iimpl_951670863_ &
+                        Core.Result.t_Result
+                          (Alloc.Vec.t_Vec Polytune.Data_types.t_Share Alloc.Alloc.t_Global &
+                            Rand_chacha.Chacha.t_ChaCha20Rng) t_Error))
+                    <:
+                    Core.Ops.Control_flow.t_ControlFlow
+                      (iimpl_951670863_ &
+                        Core.Result.t_Result
+                          (Alloc.Vec.t_Vec Polytune.Data_types.t_Share Alloc.Alloc.t_Global &
+                            Rand_chacha.Chacha.t_ChaCha20Rng) t_Error)
+                      (Prims.unit &
+                        (iimpl_951670863_ &
+                          Alloc.Vec.t_Vec (Alloc.Vec.t_Vec u128 Alloc.Alloc.t_Global)
+                            Alloc.Alloc.t_Global &
+                          Alloc.Vec.t_Vec (Alloc.Vec.t_Vec u128 Alloc.Alloc.t_Global)
+                            Alloc.Alloc.t_Global)))
                   <:
-                  t_Slice u8)
-            in
-            let c0_c1_cm:Alloc.Vec.t_Vec t_CommitmentTriple Alloc.Alloc.t_Global =
-              Alloc.Vec.impl_1__push #t_CommitmentTriple
-                #Alloc.Alloc.t_Global
-                c0_c1_cm
-                (CommitmentTriple c0 c1 cm <: t_CommitmentTriple)
-            in
-            let dmvec:Alloc.Vec.t_Vec t_VectorU8 Alloc.Alloc.t_Global =
-              Alloc.Vec.impl_1__push #t_VectorU8
-                #Alloc.Alloc.t_Global
-                dmvec
-                (VectorU8 dm <: t_VectorU8)
-            in
-            c0_c1_cm, d0, d1, dmvec
-            <:
-            (Alloc.Vec.t_Vec t_CommitmentTriple Alloc.Alloc.t_Global &
-              Alloc.Vec.t_Vec u128 Alloc.Alloc.t_Global &
-              Alloc.Vec.t_Vec u128 Alloc.Alloc.t_Global &
-              Alloc.Vec.t_Vec t_VectorU8 Alloc.Alloc.t_Global))
-    in
-    let tmp0, out:(iimpl_951670863_ &
-      Core.Result.t_Result
-        (Alloc.Vec.t_Vec (Alloc.Vec.t_Vec t_CommitmentTriple Alloc.Alloc.t_Global)
-            Alloc.Alloc.t_Global) t_Error) =
-      broadcast #t_CommitmentTriple
-        #iimpl_951670863_
-        channel
-        i
-        n
-        "fashare comm"
-        (Core.Ops.Deref.f_deref #(Alloc.Vec.t_Vec t_CommitmentTriple Alloc.Alloc.t_Global)
-            #FStar.Tactics.Typeclasses.solve
-            c0_c1_cm
-          <:
-          t_Slice t_CommitmentTriple)
-        v_RHO
-    in
-    let channel:iimpl_951670863_ = tmp0 in
-    (match
-        out
-        <:
-        Core.Result.t_Result
-          (Alloc.Vec.t_Vec (Alloc.Vec.t_Vec t_CommitmentTriple Alloc.Alloc.t_Global)
-              Alloc.Alloc.t_Global) t_Error
-      with
-      | Core.Result.Result_Ok c0_c1_cm_k ->
-        let c0_c1_cm_k:Alloc.Vec.t_Vec (Alloc.Vec.t_Vec t_CommitmentTriple Alloc.Alloc.t_Global)
+                  Core.Ops.Control_flow.t_ControlFlow
+                    (Core.Ops.Control_flow.t_ControlFlow
+                        (iimpl_951670863_ &
+                          Core.Result.t_Result
+                            (Alloc.Vec.t_Vec Polytune.Data_types.t_Share Alloc.Alloc.t_Global &
+                              Rand_chacha.Chacha.t_ChaCha20Rng) t_Error)
+                        (Prims.unit &
+                          (iimpl_951670863_ &
+                            Alloc.Vec.t_Vec (Alloc.Vec.t_Vec u128 Alloc.Alloc.t_Global)
+                              Alloc.Alloc.t_Global &
+                            Alloc.Vec.t_Vec (Alloc.Vec.t_Vec u128 Alloc.Alloc.t_Global)
+                              Alloc.Alloc.t_Global)))
+                    (iimpl_951670863_ &
+                      Alloc.Vec.t_Vec (Alloc.Vec.t_Vec u128 Alloc.Alloc.t_Global)
+                        Alloc.Alloc.t_Global &
+                      Alloc.Vec.t_Vec (Alloc.Vec.t_Vec u128 Alloc.Alloc.t_Global)
+                        Alloc.Alloc.t_Global)
+              else
+                let tmp0, out:(iimpl_951670863_ &
+                  Core.Result.t_Result
+                    (Alloc.Vec.t_Vec u128 Alloc.Alloc.t_Global & Rand_chacha.Chacha.t_ChaCha20Rng)
+                    Polytune.Swankyot.t_Error) =
+                  Polytune.Ot.kos_ot_receiver #iimpl_951670863_
+                    channel
+                    (Core.Ops.Deref.f_deref #(Alloc.Vec.t_Vec bool Alloc.Alloc.t_Global)
+                        #FStar.Tactics.Typeclasses.solve
+                        x
+                      <:
+                      t_Slice bool)
+                    k
+                    shared
+                in
+                let channel:iimpl_951670863_ = tmp0 in
+                match
+                  out
+                  <:
+                  Core.Result.t_Result
+                    (Alloc.Vec.t_Vec u128 Alloc.Alloc.t_Global & Rand_chacha.Chacha.t_ChaCha20Rng)
+                    Polytune.Swankyot.t_Error
+                with
+                | Core.Result.Result_Ok (lhs, lhs_3_) ->
+                  let macs:Alloc.Vec.t_Vec (Alloc.Vec.t_Vec u128 Alloc.Alloc.t_Global)
+                    Alloc.Alloc.t_Global =
+                    Rust_primitives.Hax.Monomorphized_update_at.update_at_usize macs k lhs
+                  in
+                  let shared_rand:Alloc.Vec.t_Vec Rand_chacha.Chacha.t_ChaCha20Rng
+                    Alloc.Alloc.t_Global =
+                    Rust_primitives.Hax.Monomorphized_update_at.update_at_usize shared_rand k lhs_3_
+                  in
+                  let _:Prims.unit = () in
+                  let tmp0, out:(iimpl_951670863_ &
+                    Core.Result.t_Result
+                      (Alloc.Vec.t_Vec u128 Alloc.Alloc.t_Global & Rand_chacha.Chacha.t_ChaCha20Rng)
+                      Polytune.Swankyot.t_Error) =
+                    Polytune.Ot.kos_ot_sender #iimpl_951670863_
+                      channel
+                      delta.Polytune.Data_types._0
+                      lprime
+                      k
+                      shared
+                  in
+                  let channel:iimpl_951670863_ = tmp0 in
+                  (match
+                      out
+                      <:
+                      Core.Result.t_Result
+                        (Alloc.Vec.t_Vec u128 Alloc.Alloc.t_Global &
+                          Rand_chacha.Chacha.t_ChaCha20Rng) Polytune.Swankyot.t_Error
+                    with
+                    | Core.Result.Result_Ok (lhs, lhs_4_) ->
+                      let keys:Alloc.Vec.t_Vec (Alloc.Vec.t_Vec u128 Alloc.Alloc.t_Global)
+                        Alloc.Alloc.t_Global =
+                        Rust_primitives.Hax.Monomorphized_update_at.update_at_usize keys k lhs
+                      in
+                      let shared_rand:Alloc.Vec.t_Vec Rand_chacha.Chacha.t_ChaCha20Rng
+                        Alloc.Alloc.t_Global =
+                        Rust_primitives.Hax.Monomorphized_update_at.update_at_usize shared_rand
+                          k
+                          lhs_4_
+                      in
+                      let _:Prims.unit = () in
+                      Core.Ops.Control_flow.ControlFlow_Continue
+                      (channel, keys, macs
+                        <:
+                        (iimpl_951670863_ &
+                          Alloc.Vec.t_Vec (Alloc.Vec.t_Vec u128 Alloc.Alloc.t_Global)
+                            Alloc.Alloc.t_Global &
+                          Alloc.Vec.t_Vec (Alloc.Vec.t_Vec u128 Alloc.Alloc.t_Global)
+                            Alloc.Alloc.t_Global))
+                      <:
+                      Core.Ops.Control_flow.t_ControlFlow
+                        (Core.Ops.Control_flow.t_ControlFlow
+                            (iimpl_951670863_ &
+                              Core.Result.t_Result
+                                (Alloc.Vec.t_Vec Polytune.Data_types.t_Share Alloc.Alloc.t_Global &
+                                  Rand_chacha.Chacha.t_ChaCha20Rng) t_Error)
+                            (Prims.unit &
+                              (iimpl_951670863_ &
+                                Alloc.Vec.t_Vec (Alloc.Vec.t_Vec u128 Alloc.Alloc.t_Global)
+                                  Alloc.Alloc.t_Global &
+                                Alloc.Vec.t_Vec (Alloc.Vec.t_Vec u128 Alloc.Alloc.t_Global)
+                                  Alloc.Alloc.t_Global)))
+                        (iimpl_951670863_ &
+                          Alloc.Vec.t_Vec (Alloc.Vec.t_Vec u128 Alloc.Alloc.t_Global)
+                            Alloc.Alloc.t_Global &
+                          Alloc.Vec.t_Vec (Alloc.Vec.t_Vec u128 Alloc.Alloc.t_Global)
+                            Alloc.Alloc.t_Global)
+                    | Core.Result.Result_Err err ->
+                      Core.Ops.Control_flow.ControlFlow_Break
+                      (Core.Ops.Control_flow.ControlFlow_Break
+                        (channel,
+                          (Core.Result.Result_Err
+                            (Core.Convert.f_from #t_Error
+                                #Polytune.Swankyot.t_Error
+                                #FStar.Tactics.Typeclasses.solve
+                                err)
+                            <:
+                            Core.Result.t_Result
+                              (Alloc.Vec.t_Vec Polytune.Data_types.t_Share Alloc.Alloc.t_Global &
+                                Rand_chacha.Chacha.t_ChaCha20Rng) t_Error)
+                          <:
+                          (iimpl_951670863_ &
+                            Core.Result.t_Result
+                              (Alloc.Vec.t_Vec Polytune.Data_types.t_Share Alloc.Alloc.t_Global &
+                                Rand_chacha.Chacha.t_ChaCha20Rng) t_Error))
+                        <:
+                        Core.Ops.Control_flow.t_ControlFlow
+                          (iimpl_951670863_ &
+                            Core.Result.t_Result
+                              (Alloc.Vec.t_Vec Polytune.Data_types.t_Share Alloc.Alloc.t_Global &
+                                Rand_chacha.Chacha.t_ChaCha20Rng) t_Error)
+                          (Prims.unit &
+                            (iimpl_951670863_ &
+                              Alloc.Vec.t_Vec (Alloc.Vec.t_Vec u128 Alloc.Alloc.t_Global)
+                                Alloc.Alloc.t_Global &
+                              Alloc.Vec.t_Vec (Alloc.Vec.t_Vec u128 Alloc.Alloc.t_Global)
+                                Alloc.Alloc.t_Global)))
+                      <:
+                      Core.Ops.Control_flow.t_ControlFlow
+                        (Core.Ops.Control_flow.t_ControlFlow
+                            (iimpl_951670863_ &
+                              Core.Result.t_Result
+                                (Alloc.Vec.t_Vec Polytune.Data_types.t_Share Alloc.Alloc.t_Global &
+                                  Rand_chacha.Chacha.t_ChaCha20Rng) t_Error)
+                            (Prims.unit &
+                              (iimpl_951670863_ &
+                                Alloc.Vec.t_Vec (Alloc.Vec.t_Vec u128 Alloc.Alloc.t_Global)
+                                  Alloc.Alloc.t_Global &
+                                Alloc.Vec.t_Vec (Alloc.Vec.t_Vec u128 Alloc.Alloc.t_Global)
+                                  Alloc.Alloc.t_Global)))
+                        (iimpl_951670863_ &
+                          Alloc.Vec.t_Vec (Alloc.Vec.t_Vec u128 Alloc.Alloc.t_Global)
+                            Alloc.Alloc.t_Global &
+                          Alloc.Vec.t_Vec (Alloc.Vec.t_Vec u128 Alloc.Alloc.t_Global)
+                            Alloc.Alloc.t_Global))
+                | Core.Result.Result_Err err ->
+                  Core.Ops.Control_flow.ControlFlow_Break
+                  (Core.Ops.Control_flow.ControlFlow_Break
+                    (channel,
+                      (Core.Result.Result_Err
+                        (Core.Convert.f_from #t_Error
+                            #Polytune.Swankyot.t_Error
+                            #FStar.Tactics.Typeclasses.solve
+                            err)
+                        <:
+                        Core.Result.t_Result
+                          (Alloc.Vec.t_Vec Polytune.Data_types.t_Share Alloc.Alloc.t_Global &
+                            Rand_chacha.Chacha.t_ChaCha20Rng) t_Error)
+                      <:
+                      (iimpl_951670863_ &
+                        Core.Result.t_Result
+                          (Alloc.Vec.t_Vec Polytune.Data_types.t_Share Alloc.Alloc.t_Global &
+                            Rand_chacha.Chacha.t_ChaCha20Rng) t_Error))
+                    <:
+                    Core.Ops.Control_flow.t_ControlFlow
+                      (iimpl_951670863_ &
+                        Core.Result.t_Result
+                          (Alloc.Vec.t_Vec Polytune.Data_types.t_Share Alloc.Alloc.t_Global &
+                            Rand_chacha.Chacha.t_ChaCha20Rng) t_Error)
+                      (Prims.unit &
+                        (iimpl_951670863_ &
+                          Alloc.Vec.t_Vec (Alloc.Vec.t_Vec u128 Alloc.Alloc.t_Global)
+                            Alloc.Alloc.t_Global &
+                          Alloc.Vec.t_Vec (Alloc.Vec.t_Vec u128 Alloc.Alloc.t_Global)
+                            Alloc.Alloc.t_Global)))
+                  <:
+                  Core.Ops.Control_flow.t_ControlFlow
+                    (Core.Ops.Control_flow.t_ControlFlow
+                        (iimpl_951670863_ &
+                          Core.Result.t_Result
+                            (Alloc.Vec.t_Vec Polytune.Data_types.t_Share Alloc.Alloc.t_Global &
+                              Rand_chacha.Chacha.t_ChaCha20Rng) t_Error)
+                        (Prims.unit &
+                          (iimpl_951670863_ &
+                            Alloc.Vec.t_Vec (Alloc.Vec.t_Vec u128 Alloc.Alloc.t_Global)
+                              Alloc.Alloc.t_Global &
+                            Alloc.Vec.t_Vec (Alloc.Vec.t_Vec u128 Alloc.Alloc.t_Global)
+                              Alloc.Alloc.t_Global)))
+                    (iimpl_951670863_ &
+                      Alloc.Vec.t_Vec (Alloc.Vec.t_Vec u128 Alloc.Alloc.t_Global)
+                        Alloc.Alloc.t_Global &
+                      Alloc.Vec.t_Vec (Alloc.Vec.t_Vec u128 Alloc.Alloc.t_Global)
+                        Alloc.Alloc.t_Global))
+      <:
+      Core.Ops.Control_flow.t_ControlFlow
+        (iimpl_951670863_ &
+          Core.Result.t_Result
+            (Alloc.Vec.t_Vec Polytune.Data_types.t_Share Alloc.Alloc.t_Global &
+              Rand_chacha.Chacha.t_ChaCha20Rng) t_Error)
+        (iimpl_951670863_ &
+          Alloc.Vec.t_Vec (Alloc.Vec.t_Vec u128 Alloc.Alloc.t_Global) Alloc.Alloc.t_Global &
+          Alloc.Vec.t_Vec (Alloc.Vec.t_Vec u128 Alloc.Alloc.t_Global) Alloc.Alloc.t_Global)
+    with
+    | Core.Ops.Control_flow.ControlFlow_Break ret -> ret
+    | Core.Ops.Control_flow.ControlFlow_Continue (channel, keys, macs) ->
+      let tmp0, out:(iimpl_951670863_ &
+        Core.Result.t_Result Rand_chacha.Chacha.t_ChaCha20Rng t_Error) =
+        shared_rng #iimpl_951670863_ channel i n
+      in
+      let channel:iimpl_951670863_ = tmp0 in
+      match out <: Core.Result.t_Result Rand_chacha.Chacha.t_ChaCha20Rng t_Error with
+      | Core.Result.Result_Ok multi_shared_rand ->
+        let r:Alloc.Vec.t_Vec (Alloc.Vec.t_Vec bool Alloc.Alloc.t_Global) Alloc.Alloc.t_Global =
+          Alloc.Vec.impl__with_capacity #(Alloc.Vec.t_Vec bool Alloc.Alloc.t_Global) three_rho
+        in
+        let multi_shared_rand, r:(Rand_chacha.Chacha.t_ChaCha20Rng &
+          Alloc.Vec.t_Vec (Alloc.Vec.t_Vec bool Alloc.Alloc.t_Global) Alloc.Alloc.t_Global) =
+          Rust_primitives.Hax.Folds.fold_range (mk_usize 0)
+            three_rho
+            (fun temp_0_ temp_1_ ->
+                let multi_shared_rand, r:(Rand_chacha.Chacha.t_ChaCha20Rng &
+                  Alloc.Vec.t_Vec (Alloc.Vec.t_Vec bool Alloc.Alloc.t_Global) Alloc.Alloc.t_Global)
+                =
+                  temp_0_
+                in
+                let _:usize = temp_1_ in
+                true)
+            (multi_shared_rand, r
+              <:
+              (Rand_chacha.Chacha.t_ChaCha20Rng &
+                Alloc.Vec.t_Vec (Alloc.Vec.t_Vec bool Alloc.Alloc.t_Global) Alloc.Alloc.t_Global))
+            (fun temp_0_ temp_1_ ->
+                let multi_shared_rand, r:(Rand_chacha.Chacha.t_ChaCha20Rng &
+                  Alloc.Vec.t_Vec (Alloc.Vec.t_Vec bool Alloc.Alloc.t_Global) Alloc.Alloc.t_Global)
+                =
+                  temp_0_
+                in
+                let _:usize = temp_1_ in
+                let inner:Alloc.Vec.t_Vec bool Alloc.Alloc.t_Global =
+                  Alloc.Vec.impl__with_capacity #bool lprime
+                in
+                let inner, multi_shared_rand:(Alloc.Vec.t_Vec bool Alloc.Alloc.t_Global &
+                  Rand_chacha.Chacha.t_ChaCha20Rng) =
+                  Rust_primitives.Hax.Folds.fold_range (mk_usize 0)
+                    lprime
+                    (fun temp_0_ temp_1_ ->
+                        let inner, multi_shared_rand:(Alloc.Vec.t_Vec bool Alloc.Alloc.t_Global &
+                          Rand_chacha.Chacha.t_ChaCha20Rng) =
+                          temp_0_
+                        in
+                        let _:usize = temp_1_ in
+                        true)
+                    (inner, multi_shared_rand
+                      <:
+                      (Alloc.Vec.t_Vec bool Alloc.Alloc.t_Global & Rand_chacha.Chacha.t_ChaCha20Rng)
+                    )
+                    (fun temp_0_ temp_1_ ->
+                        let inner, multi_shared_rand:(Alloc.Vec.t_Vec bool Alloc.Alloc.t_Global &
+                          Rand_chacha.Chacha.t_ChaCha20Rng) =
+                          temp_0_
+                        in
+                        let _:usize = temp_1_ in
+                        let tmp0, out:(Rand_chacha.Chacha.t_ChaCha20Rng & bool) =
+                          Rand.Rng.f_gen #Rand_chacha.Chacha.t_ChaCha20Rng
+                            #FStar.Tactics.Typeclasses.solve
+                            #bool
+                            multi_shared_rand
+                        in
+                        let multi_shared_rand:Rand_chacha.Chacha.t_ChaCha20Rng = tmp0 in
+                        Alloc.Vec.impl_1__push #bool #Alloc.Alloc.t_Global inner out,
+                        multi_shared_rand
+                        <:
+                        (Alloc.Vec.t_Vec bool Alloc.Alloc.t_Global &
+                          Rand_chacha.Chacha.t_ChaCha20Rng))
+                in
+                let r:Alloc.Vec.t_Vec (Alloc.Vec.t_Vec bool Alloc.Alloc.t_Global)
+                  Alloc.Alloc.t_Global =
+                  Alloc.Vec.impl_1__push #(Alloc.Vec.t_Vec bool Alloc.Alloc.t_Global)
+                    #Alloc.Alloc.t_Global
+                    r
+                    inner
+                in
+                multi_shared_rand, r
+                <:
+                (Rand_chacha.Chacha.t_ChaCha20Rng &
+                  Alloc.Vec.t_Vec (Alloc.Vec.t_Vec bool Alloc.Alloc.t_Global) Alloc.Alloc.t_Global))
+        in
+        let xj:Alloc.Vec.t_Vec bool Alloc.Alloc.t_Global =
+          Alloc.Vec.impl__with_capacity #bool three_rho
+        in
+        let xj:Alloc.Vec.t_Vec bool Alloc.Alloc.t_Global =
+          Core.Iter.Traits.Iterator.f_fold (Core.Iter.Traits.Collect.f_into_iter #(Alloc.Vec.t_Vec
+                    (Alloc.Vec.t_Vec bool Alloc.Alloc.t_Global) Alloc.Alloc.t_Global)
+                #FStar.Tactics.Typeclasses.solve
+                r
+              <:
+              Core.Slice.Iter.t_Iter (Alloc.Vec.t_Vec bool Alloc.Alloc.t_Global))
+            xj
+            (fun xj rbits ->
+                let xj:Alloc.Vec.t_Vec bool Alloc.Alloc.t_Global = xj in
+                let rbits:Alloc.Vec.t_Vec bool Alloc.Alloc.t_Global = rbits in
+                let xm:bool = false in
+                let xm:bool =
+                  Core.Iter.Traits.Iterator.f_fold (Core.Iter.Traits.Collect.f_into_iter #(Core.Iter.Adapters.Zip.t_Zip
+                            (Core.Slice.Iter.t_Iter bool) (Core.Slice.Iter.t_Iter bool))
+                        #FStar.Tactics.Typeclasses.solve
+                        (Core.Iter.Traits.Iterator.f_zip #(Core.Slice.Iter.t_Iter bool)
+                            #FStar.Tactics.Typeclasses.solve
+                            #(Alloc.Vec.t_Vec bool Alloc.Alloc.t_Global)
+                            (Core.Slice.impl__iter #bool
+                                (Core.Ops.Deref.f_deref #(Alloc.Vec.t_Vec bool Alloc.Alloc.t_Global)
+                                    #FStar.Tactics.Typeclasses.solve
+                                    x
+                                  <:
+                                  t_Slice bool)
+                              <:
+                              Core.Slice.Iter.t_Iter bool)
+                            rbits
+                          <:
+                          Core.Iter.Adapters.Zip.t_Zip (Core.Slice.Iter.t_Iter bool)
+                            (Core.Slice.Iter.t_Iter bool))
+                      <:
+                      Core.Iter.Adapters.Zip.t_Zip (Core.Slice.Iter.t_Iter bool)
+                        (Core.Slice.Iter.t_Iter bool))
+                    xm
+                    (fun xm temp_1_ ->
+                        let xm:bool = xm in
+                        let xi, ri:(bool & bool) = temp_1_ in
+                        Core.Ops.Bit.f_bitxor xm
+                          (Core.Ops.Bit.f_bitand #bool #bool #FStar.Tactics.Typeclasses.solve xi ri
+                            <:
+                            bool)
+                        <:
+                        bool)
+                in
+                let xj:Alloc.Vec.t_Vec bool Alloc.Alloc.t_Global =
+                  Alloc.Vec.impl_1__push #bool #Alloc.Alloc.t_Global xj xm
+                in
+                xj)
+        in
+        let xj_xjmac:Alloc.Vec.t_Vec (Alloc.Vec.t_Vec (bool & u128) Alloc.Alloc.t_Global)
           Alloc.Alloc.t_Global =
-          Rust_primitives.Hax.Monomorphized_update_at.update_at_usize c0_c1_cm_k i c0_c1_cm
+          Alloc.Vec.from_elem #(Alloc.Vec.t_Vec (bool & u128) Alloc.Alloc.t_Global)
+            (Alloc.Vec.impl__new #(bool & u128) ()
+              <:
+              Alloc.Vec.t_Vec (bool & u128) Alloc.Alloc.t_Global)
+            n
+        in
+        let xj_xjmac:Alloc.Vec.t_Vec (Alloc.Vec.t_Vec (bool & u128) Alloc.Alloc.t_Global)
+          Alloc.Alloc.t_Global =
+          Rust_primitives.Hax.Folds.fold_range (mk_usize 0)
+            n
+            (fun xj_xjmac temp_1_ ->
+                let xj_xjmac:Alloc.Vec.t_Vec (Alloc.Vec.t_Vec (bool & u128) Alloc.Alloc.t_Global)
+                  Alloc.Alloc.t_Global =
+                  xj_xjmac
+                in
+                let _:usize = temp_1_ in
+                true)
+            xj_xjmac
+            (fun xj_xjmac k ->
+                let xj_xjmac:Alloc.Vec.t_Vec (Alloc.Vec.t_Vec (bool & u128) Alloc.Alloc.t_Global)
+                  Alloc.Alloc.t_Global =
+                  xj_xjmac
+                in
+                let k:usize = k in
+                if k =. i <: bool
+                then xj_xjmac
+                else
+                  Core.Iter.Traits.Iterator.f_fold (Core.Iter.Traits.Collect.f_into_iter #(Core.Iter.Adapters.Zip.t_Zip
+                            (Core.Slice.Iter.t_Iter (Alloc.Vec.t_Vec bool Alloc.Alloc.t_Global))
+                            (Core.Slice.Iter.t_Iter bool))
+                        #FStar.Tactics.Typeclasses.solve
+                        (Core.Iter.Traits.Iterator.f_zip #(Core.Slice.Iter.t_Iter
+                              (Alloc.Vec.t_Vec bool Alloc.Alloc.t_Global))
+                            #FStar.Tactics.Typeclasses.solve
+                            #(Core.Slice.Iter.t_Iter bool)
+                            (Core.Slice.impl__iter #(Alloc.Vec.t_Vec bool Alloc.Alloc.t_Global)
+                                (Core.Ops.Deref.f_deref #(Alloc.Vec.t_Vec
+                                        (Alloc.Vec.t_Vec bool Alloc.Alloc.t_Global)
+                                        Alloc.Alloc.t_Global)
+                                    #FStar.Tactics.Typeclasses.solve
+                                    r
+                                  <:
+                                  t_Slice (Alloc.Vec.t_Vec bool Alloc.Alloc.t_Global))
+                              <:
+                              Core.Slice.Iter.t_Iter (Alloc.Vec.t_Vec bool Alloc.Alloc.t_Global))
+                            (Core.Slice.impl__iter #bool
+                                (Core.Ops.Deref.f_deref #(Alloc.Vec.t_Vec bool Alloc.Alloc.t_Global)
+                                    #FStar.Tactics.Typeclasses.solve
+                                    xj
+                                  <:
+                                  t_Slice bool)
+                              <:
+                              Core.Slice.Iter.t_Iter bool)
+                          <:
+                          Core.Iter.Adapters.Zip.t_Zip
+                            (Core.Slice.Iter.t_Iter (Alloc.Vec.t_Vec bool Alloc.Alloc.t_Global))
+                            (Core.Slice.Iter.t_Iter bool))
+                      <:
+                      Core.Iter.Adapters.Zip.t_Zip
+                        (Core.Slice.Iter.t_Iter (Alloc.Vec.t_Vec bool Alloc.Alloc.t_Global))
+                        (Core.Slice.Iter.t_Iter bool))
+                    xj_xjmac
+                    (fun xj_xjmac temp_1_ ->
+                        let xj_xjmac:Alloc.Vec.t_Vec
+                          (Alloc.Vec.t_Vec (bool & u128) Alloc.Alloc.t_Global) Alloc.Alloc.t_Global
+                        =
+                          xj_xjmac
+                        in
+                        let rbits, xj:(Alloc.Vec.t_Vec bool Alloc.Alloc.t_Global & bool) =
+                          temp_1_
+                        in
+                        let xjmac:u128 = mk_u128 0 in
+                        let xjmac:u128 =
+                          Rust_primitives.Hax.Folds.fold_enumerated_slice (Core.Ops.Deref.f_deref #(Alloc.Vec.t_Vec
+                                    bool Alloc.Alloc.t_Global)
+                                #FStar.Tactics.Typeclasses.solve
+                                rbits
+                              <:
+                              t_Slice bool)
+                            (fun xjmac temp_1_ ->
+                                let xjmac:u128 = xjmac in
+                                let _:usize = temp_1_ in
+                                true)
+                            xjmac
+                            (fun xjmac temp_1_ ->
+                                let xjmac:u128 = xjmac in
+                                let j, rbit:(usize & bool) = temp_1_ in
+                                if rbit
+                                then
+                                  let xjmac:u128 =
+                                    xjmac ^.
+                                    ((macs.[ k ] <: Alloc.Vec.t_Vec u128 Alloc.Alloc.t_Global).[ j ]
+                                      <:
+                                      u128)
+                                  in
+                                  xjmac
+                                else xjmac)
+                        in
+                        let xj_xjmac:Alloc.Vec.t_Vec
+                          (Alloc.Vec.t_Vec (bool & u128) Alloc.Alloc.t_Global) Alloc.Alloc.t_Global
+                        =
+                          Rust_primitives.Hax.Monomorphized_update_at.update_at_usize xj_xjmac
+                            k
+                            (Alloc.Vec.impl_1__push #(bool & u128)
+                                #Alloc.Alloc.t_Global
+                                (xj_xjmac.[ k ]
+                                  <:
+                                  Alloc.Vec.t_Vec (bool & u128) Alloc.Alloc.t_Global)
+                                (xj, xjmac <: (bool & u128))
+                              <:
+                              Alloc.Vec.t_Vec (bool & u128) Alloc.Alloc.t_Global)
+                        in
+                        xj_xjmac)
+                  <:
+                  Alloc.Vec.t_Vec (Alloc.Vec.t_Vec (bool & u128) Alloc.Alloc.t_Global)
+                    Alloc.Alloc.t_Global)
         in
         let tmp0, out:(iimpl_951670863_ &
           Core.Result.t_Result
-            (Alloc.Vec.t_Vec (Alloc.Vec.t_Vec t_VectorU8 Alloc.Alloc.t_Global) Alloc.Alloc.t_Global)
-            t_Error) =
-          broadcast #t_VectorU8
+            (Alloc.Vec.t_Vec (Alloc.Vec.t_Vec (bool & u128) Alloc.Alloc.t_Global)
+                Alloc.Alloc.t_Global) t_Error) =
+          broadcast_first_send_second #bool
+            #u128
             #iimpl_951670863_
             channel
             i
             n
-            "fashare ver"
-            (Core.Ops.Deref.f_deref #(Alloc.Vec.t_Vec t_VectorU8 Alloc.Alloc.t_Global)
+            "fabitn"
+            (Core.Ops.Deref.f_deref #(Alloc.Vec.t_Vec
+                    (Alloc.Vec.t_Vec (bool & u128) Alloc.Alloc.t_Global) Alloc.Alloc.t_Global)
                 #FStar.Tactics.Typeclasses.solve
-                dmvec
+                xj_xjmac
               <:
-              t_Slice t_VectorU8)
-            v_RHO
+              t_Slice (Alloc.Vec.t_Vec (bool & u128) Alloc.Alloc.t_Global))
+            three_rho
         in
         let channel:iimpl_951670863_ = tmp0 in
         (match
             out
             <:
             Core.Result.t_Result
-              (Alloc.Vec.t_Vec (Alloc.Vec.t_Vec t_VectorU8 Alloc.Alloc.t_Global)
+              (Alloc.Vec.t_Vec (Alloc.Vec.t_Vec (bool & u128) Alloc.Alloc.t_Global)
                   Alloc.Alloc.t_Global) t_Error
           with
-          | Core.Result.Result_Ok dm_k ->
-            let dm_k:Alloc.Vec.t_Vec (Alloc.Vec.t_Vec t_VectorU8 Alloc.Alloc.t_Global)
-              Alloc.Alloc.t_Global =
-              Rust_primitives.Hax.Monomorphized_update_at.update_at_usize dm_k i dmvec
-            in
-            let (bi: t_Array u8 (mk_usize 40)):t_Array u8 (mk_usize 40) =
-              Rust_primitives.Hax.repeat (mk_u8 0) (mk_usize 40)
-            in
-            let (di_bi: Alloc.Vec.t_Vec u128 Alloc.Alloc.t_Global):Alloc.Vec.t_Vec u128
-              Alloc.Alloc.t_Global =
-              Alloc.Vec.from_elem #u128 (mk_u128 0) v_RHO
-            in
+          | Core.Result.Result_Ok xj_xjmac_k ->
             (match
-                Rust_primitives.Hax.Folds.fold_range_return (mk_usize 0)
-                  v_RHO
+                Rust_primitives.Hax.Folds.fold_enumerated_slice_return (Core.Ops.Deref.f_deref #(Alloc.Vec.t_Vec
+                          (Alloc.Vec.t_Vec bool Alloc.Alloc.t_Global) Alloc.Alloc.t_Global)
+                      #FStar.Tactics.Typeclasses.solve
+                      r
+                    <:
+                    t_Slice (Alloc.Vec.t_Vec bool Alloc.Alloc.t_Global))
                   (fun temp_0_ temp_1_ ->
-                      let bi, di_bi:(t_Array u8 (mk_usize 40) &
-                        Alloc.Vec.t_Vec u128 Alloc.Alloc.t_Global) =
-                        temp_0_
-                      in
+                      let _:Prims.unit = temp_0_ in
                       let _:usize = temp_1_ in
                       true)
-                  (bi, di_bi
-                    <:
-                    (t_Array u8 (mk_usize 40) & Alloc.Vec.t_Vec u128 Alloc.Alloc.t_Global))
-                  (fun temp_0_ r ->
-                      let bi, di_bi:(t_Array u8 (mk_usize 40) &
-                        Alloc.Vec.t_Vec u128 Alloc.Alloc.t_Global) =
-                        temp_0_
-                      in
-                      let r:usize = r in
+                  ()
+                  (fun temp_0_ temp_1_ ->
+                      let _:Prims.unit = temp_0_ in
+                      let j, rbits:(usize & Alloc.Vec.t_Vec bool Alloc.Alloc.t_Global) = temp_1_ in
                       match
                         Rust_primitives.Hax.Folds.fold_range_return (mk_usize 0)
                           n
-                          (fun bi temp_1_ ->
-                              let bi:t_Array u8 (mk_usize 40) = bi in
+                          (fun temp_0_ temp_1_ ->
+                              let _:Prims.unit = temp_0_ in
                               let _:usize = temp_1_ in
                               true)
-                          bi
-                          (fun bi k ->
-                              let bi:t_Array u8 (mk_usize 40) = bi in
+                          ()
+                          (fun temp_0_ k ->
+                              let _:Prims.unit = temp_0_ in
                               let k:usize = k in
                               if k =. i <: bool
                               then
-                                Core.Ops.Control_flow.ControlFlow_Continue bi
+                                Core.Ops.Control_flow.ControlFlow_Continue (() <: Prims.unit)
                                 <:
                                 Core.Ops.Control_flow.t_ControlFlow
                                   (Core.Ops.Control_flow.t_ControlFlow
@@ -519,25 +954,50 @@ let fashare
                                           (Alloc.Vec.t_Vec Polytune.Data_types.t_Share
                                               Alloc.Alloc.t_Global &
                                             Rand_chacha.Chacha.t_ChaCha20Rng) t_Error)
-                                      (Prims.unit & t_Array u8 (mk_usize 40)))
-                                  (t_Array u8 (mk_usize 40))
+                                      (Prims.unit & Prims.unit)) Prims.unit
                               else
-                                if
-                                  (((dm_k.[ k ] <: Alloc.Vec.t_Vec t_VectorU8 Alloc.Alloc.t_Global).[
-                                        r ]
-                                      <:
-                                      t_VectorU8)
-                                      ._0.[ mk_usize 0 ]
+                                let xj, xjmac:(bool & u128) =
+                                  (xj_xjmac_k.[ k ]
                                     <:
-                                    u8) >.
-                                  mk_u8 1
-                                  <:
-                                  bool
+                                    Alloc.Vec.t_Vec (bool & u128) Alloc.Alloc.t_Global).[ j ]
+                                in
+                                let xjkey:u128 = mk_u128 0 in
+                                let xjkey:u128 =
+                                  Rust_primitives.Hax.Folds.fold_enumerated_slice (Core.Ops.Deref.f_deref
+                                        #(Alloc.Vec.t_Vec bool Alloc.Alloc.t_Global)
+                                        #FStar.Tactics.Typeclasses.solve
+                                        rbits
+                                      <:
+                                      t_Slice bool)
+                                    (fun xjkey temp_1_ ->
+                                        let xjkey:u128 = xjkey in
+                                        let _:usize = temp_1_ in
+                                        true)
+                                    xjkey
+                                    (fun xjkey temp_1_ ->
+                                        let xjkey:u128 = xjkey in
+                                        let i, rbit:(usize & bool) = temp_1_ in
+                                        if rbit
+                                        then
+                                          let xjkey:u128 =
+                                            xjkey ^.
+                                            ((keys.[ k ]
+                                                <:
+                                                Alloc.Vec.t_Vec u128 Alloc.Alloc.t_Global).[ i ]
+                                              <:
+                                              u128)
+                                          in
+                                          xjkey
+                                        else xjkey)
+                                in
+                                if
+                                  xj && xjmac <>. (xjkey ^. delta.Polytune.Data_types._0 <: u128) ||
+                                  ~.xj && xjmac <>. xjkey
                                 then
                                   Core.Ops.Control_flow.ControlFlow_Break
                                   (Core.Ops.Control_flow.ControlFlow_Break
                                     (channel,
-                                      (Core.Result.Result_Err (Error_InvalidBitValue <: t_Error)
+                                      (Core.Result.Result_Err (Error_ABitWrongMAC <: t_Error)
                                         <:
                                         Core.Result.t_Result
                                           (Alloc.Vec.t_Vec Polytune.Data_types.t_Share
@@ -556,7 +1016,7 @@ let fashare
                                           (Alloc.Vec.t_Vec Polytune.Data_types.t_Share
                                               Alloc.Alloc.t_Global &
                                             Rand_chacha.Chacha.t_ChaCha20Rng) t_Error)
-                                      (Prims.unit & t_Array u8 (mk_usize 40)))
+                                      (Prims.unit & Prims.unit))
                                   <:
                                   Core.Ops.Control_flow.t_ControlFlow
                                     (Core.Ops.Control_flow.t_ControlFlow
@@ -565,30 +1025,9 @@ let fashare
                                             (Alloc.Vec.t_Vec Polytune.Data_types.t_Share
                                                 Alloc.Alloc.t_Global &
                                               Rand_chacha.Chacha.t_ChaCha20Rng) t_Error)
-                                        (Prims.unit & t_Array u8 (mk_usize 40)))
-                                    (t_Array u8 (mk_usize 40))
+                                        (Prims.unit & Prims.unit)) Prims.unit
                                 else
-                                  let cond:u8 = mk_u8 0 in
-                                  let cond:u8 =
-                                    if
-                                      (((dm_k.[ k ]
-                                            <:
-                                            Alloc.Vec.t_Vec t_VectorU8 Alloc.Alloc.t_Global).[ r ]
-                                          <:
-                                          t_VectorU8)
-                                          ._0.[ mk_usize 0 ]
-                                        <:
-                                        u8) <>.
-                                      mk_u8 0
-                                    then
-                                      let cond:u8 = mk_u8 1 in
-                                      cond
-                                    else cond
-                                  in
-                                  Core.Ops.Control_flow.ControlFlow_Continue
-                                  (Rust_primitives.Hax.Monomorphized_update_at.update_at_usize bi
-                                      r
-                                      ((bi.[ r ] <: u8) ^. cond <: u8))
+                                  Core.Ops.Control_flow.ControlFlow_Continue ()
                                   <:
                                   Core.Ops.Control_flow.t_ControlFlow
                                     (Core.Ops.Control_flow.t_ControlFlow
@@ -597,15 +1036,13 @@ let fashare
                                             (Alloc.Vec.t_Vec Polytune.Data_types.t_Share
                                                 Alloc.Alloc.t_Global &
                                               Rand_chacha.Chacha.t_ChaCha20Rng) t_Error)
-                                        (Prims.unit & t_Array u8 (mk_usize 40)))
-                                    (t_Array u8 (mk_usize 40)))
+                                        (Prims.unit & Prims.unit)) Prims.unit)
                         <:
                         Core.Ops.Control_flow.t_ControlFlow
                           (iimpl_951670863_ &
                             Core.Result.t_Result
                               (Alloc.Vec.t_Vec Polytune.Data_types.t_Share Alloc.Alloc.t_Global &
-                                Rand_chacha.Chacha.t_ChaCha20Rng) t_Error)
-                          (t_Array u8 (mk_usize 40))
+                                Rand_chacha.Chacha.t_ChaCha20Rng) t_Error) Prims.unit
                       with
                       | Core.Ops.Control_flow.ControlFlow_Break ret ->
                         Core.Ops.Control_flow.ControlFlow_Break
@@ -616,9 +1053,7 @@ let fashare
                               Core.Result.t_Result
                                 (Alloc.Vec.t_Vec Polytune.Data_types.t_Share Alloc.Alloc.t_Global &
                                   Rand_chacha.Chacha.t_ChaCha20Rng) t_Error)
-                            (Prims.unit &
-                              (t_Array u8 (mk_usize 40) & Alloc.Vec.t_Vec u128 Alloc.Alloc.t_Global)
-                            ))
+                            (Prims.unit & Prims.unit))
                         <:
                         Core.Ops.Control_flow.t_ControlFlow
                           (Core.Ops.Control_flow.t_ControlFlow
@@ -626,22 +1061,9 @@ let fashare
                                 Core.Result.t_Result
                                   (Alloc.Vec.t_Vec Polytune.Data_types.t_Share Alloc.Alloc.t_Global &
                                     Rand_chacha.Chacha.t_ChaCha20Rng) t_Error)
-                              (Prims.unit &
-                                (t_Array u8 (mk_usize 40) &
-                                  Alloc.Vec.t_Vec u128 Alloc.Alloc.t_Global)))
-                          (t_Array u8 (mk_usize 40) & Alloc.Vec.t_Vec u128 Alloc.Alloc.t_Global)
-                      | Core.Ops.Control_flow.ControlFlow_Continue bi ->
-                        let di_bi:Alloc.Vec.t_Vec u128 Alloc.Alloc.t_Global =
-                          Rust_primitives.Hax.Monomorphized_update_at.update_at_usize di_bi
-                            r
-                            (if (bi.[ r ] <: u8) =. mk_u8 1 <: bool
-                              then d1.[ r ] <: u128
-                              else d0.[ r ] <: u128)
-                        in
-                        Core.Ops.Control_flow.ControlFlow_Continue
-                        (bi, di_bi
-                          <:
-                          (t_Array u8 (mk_usize 40) & Alloc.Vec.t_Vec u128 Alloc.Alloc.t_Global))
+                              (Prims.unit & Prims.unit)) Prims.unit
+                      | Core.Ops.Control_flow.ControlFlow_Continue loop_res ->
+                        Core.Ops.Control_flow.ControlFlow_Continue loop_res
                         <:
                         Core.Ops.Control_flow.t_ControlFlow
                           (Core.Ops.Control_flow.t_ControlFlow
@@ -649,673 +1071,213 @@ let fashare
                                 Core.Result.t_Result
                                   (Alloc.Vec.t_Vec Polytune.Data_types.t_Share Alloc.Alloc.t_Global &
                                     Rand_chacha.Chacha.t_ChaCha20Rng) t_Error)
-                              (Prims.unit &
-                                (t_Array u8 (mk_usize 40) &
-                                  Alloc.Vec.t_Vec u128 Alloc.Alloc.t_Global)))
-                          (t_Array u8 (mk_usize 40) & Alloc.Vec.t_Vec u128 Alloc.Alloc.t_Global))
+                              (Prims.unit & Prims.unit)) Prims.unit)
                 <:
                 Core.Ops.Control_flow.t_ControlFlow
                   (iimpl_951670863_ &
                     Core.Result.t_Result
                       (Alloc.Vec.t_Vec Polytune.Data_types.t_Share Alloc.Alloc.t_Global &
-                        Rand_chacha.Chacha.t_ChaCha20Rng) t_Error)
-                  (t_Array u8 (mk_usize 40) & Alloc.Vec.t_Vec u128 Alloc.Alloc.t_Global)
+                        Rand_chacha.Chacha.t_ChaCha20Rng) t_Error) Prims.unit
               with
               | Core.Ops.Control_flow.ControlFlow_Break ret -> ret
-              | Core.Ops.Control_flow.ControlFlow_Continue (bi, di_bi) ->
-                let tmp0, out:(iimpl_951670863_ &
-                  Core.Result.t_Result
-                    (Alloc.Vec.t_Vec (Alloc.Vec.t_Vec u128 Alloc.Alloc.t_Global)
-                        Alloc.Alloc.t_Global) t_Error) =
-                  broadcast #u128
-                    #iimpl_951670863_
-                    channel
-                    i
-                    n
-                    "fashare di_bi"
-                    (Core.Ops.Deref.f_deref #(Alloc.Vec.t_Vec u128 Alloc.Alloc.t_Global)
-                        #FStar.Tactics.Typeclasses.solve
-                        di_bi
-                      <:
-                      t_Slice u128)
-                    v_RHO
+              | Core.Ops.Control_flow.ControlFlow_Continue _ ->
+                let _:Prims.unit =
+                  Core.Mem.drop #(Alloc.Vec.t_Vec (Alloc.Vec.t_Vec bool Alloc.Alloc.t_Global)
+                        Alloc.Alloc.t_Global)
+                    r
                 in
-                let channel:iimpl_951670863_ = tmp0 in
-                match
-                  out
+                let x:Alloc.Vec.t_Vec bool Alloc.Alloc.t_Global =
+                  Alloc.Vec.impl_1__truncate #bool #Alloc.Alloc.t_Global x l
+                in
+                let keys, macs:(Alloc.Vec.t_Vec (Alloc.Vec.t_Vec u128 Alloc.Alloc.t_Global)
+                    Alloc.Alloc.t_Global &
+                  Alloc.Vec.t_Vec (Alloc.Vec.t_Vec u128 Alloc.Alloc.t_Global) Alloc.Alloc.t_Global)
+                =
+                  Rust_primitives.Hax.Folds.fold_range (mk_usize 0)
+                    n
+                    (fun temp_0_ temp_1_ ->
+                        let keys, macs:(Alloc.Vec.t_Vec (Alloc.Vec.t_Vec u128 Alloc.Alloc.t_Global)
+                            Alloc.Alloc.t_Global &
+                          Alloc.Vec.t_Vec (Alloc.Vec.t_Vec u128 Alloc.Alloc.t_Global)
+                            Alloc.Alloc.t_Global) =
+                          temp_0_
+                        in
+                        let _:usize = temp_1_ in
+                        true)
+                    (keys, macs
+                      <:
+                      (Alloc.Vec.t_Vec (Alloc.Vec.t_Vec u128 Alloc.Alloc.t_Global)
+                          Alloc.Alloc.t_Global &
+                        Alloc.Vec.t_Vec (Alloc.Vec.t_Vec u128 Alloc.Alloc.t_Global)
+                          Alloc.Alloc.t_Global))
+                    (fun temp_0_ k ->
+                        let keys, macs:(Alloc.Vec.t_Vec (Alloc.Vec.t_Vec u128 Alloc.Alloc.t_Global)
+                            Alloc.Alloc.t_Global &
+                          Alloc.Vec.t_Vec (Alloc.Vec.t_Vec u128 Alloc.Alloc.t_Global)
+                            Alloc.Alloc.t_Global) =
+                          temp_0_
+                        in
+                        let k:usize = k in
+                        if k =. i <: bool
+                        then
+                          keys, macs
+                          <:
+                          (Alloc.Vec.t_Vec (Alloc.Vec.t_Vec u128 Alloc.Alloc.t_Global)
+                              Alloc.Alloc.t_Global &
+                            Alloc.Vec.t_Vec (Alloc.Vec.t_Vec u128 Alloc.Alloc.t_Global)
+                              Alloc.Alloc.t_Global)
+                        else
+                          let keys:Alloc.Vec.t_Vec (Alloc.Vec.t_Vec u128 Alloc.Alloc.t_Global)
+                            Alloc.Alloc.t_Global =
+                            Rust_primitives.Hax.Monomorphized_update_at.update_at_usize keys
+                              k
+                              (Alloc.Vec.impl_1__truncate #u128
+                                  #Alloc.Alloc.t_Global
+                                  (keys.[ k ] <: Alloc.Vec.t_Vec u128 Alloc.Alloc.t_Global)
+                                  l
+                                <:
+                                Alloc.Vec.t_Vec u128 Alloc.Alloc.t_Global)
+                          in
+                          let macs:Alloc.Vec.t_Vec (Alloc.Vec.t_Vec u128 Alloc.Alloc.t_Global)
+                            Alloc.Alloc.t_Global =
+                            Rust_primitives.Hax.Monomorphized_update_at.update_at_usize macs
+                              k
+                              (Alloc.Vec.impl_1__truncate #u128
+                                  #Alloc.Alloc.t_Global
+                                  (macs.[ k ] <: Alloc.Vec.t_Vec u128 Alloc.Alloc.t_Global)
+                                  l
+                                <:
+                                Alloc.Vec.t_Vec u128 Alloc.Alloc.t_Global)
+                          in
+                          keys, macs
+                          <:
+                          (Alloc.Vec.t_Vec (Alloc.Vec.t_Vec u128 Alloc.Alloc.t_Global)
+                              Alloc.Alloc.t_Global &
+                            Alloc.Vec.t_Vec (Alloc.Vec.t_Vec u128 Alloc.Alloc.t_Global)
+                              Alloc.Alloc.t_Global))
+                in
+                let res:Alloc.Vec.t_Vec Polytune.Data_types.t_Share Alloc.Alloc.t_Global =
+                  Alloc.Vec.impl__with_capacity #Polytune.Data_types.t_Share l
+                in
+                let res:Alloc.Vec.t_Vec Polytune.Data_types.t_Share Alloc.Alloc.t_Global =
+                  Core.Iter.Traits.Iterator.f_fold (Core.Iter.Traits.Collect.f_into_iter #(Core.Iter.Adapters.Take.t_Take
+                          (Core.Iter.Adapters.Enumerate.t_Enumerate (Core.Slice.Iter.t_Iter bool)))
+                        #FStar.Tactics.Typeclasses.solve
+                        (Core.Iter.Traits.Iterator.f_take #(Core.Iter.Adapters.Enumerate.t_Enumerate
+                              (Core.Slice.Iter.t_Iter bool))
+                            #FStar.Tactics.Typeclasses.solve
+                            (Core.Iter.Traits.Iterator.f_enumerate #(Core.Slice.Iter.t_Iter bool)
+                                #FStar.Tactics.Typeclasses.solve
+                                (Core.Slice.impl__iter #bool
+                                    (Core.Ops.Deref.f_deref #(Alloc.Vec.t_Vec bool
+                                            Alloc.Alloc.t_Global)
+                                        #FStar.Tactics.Typeclasses.solve
+                                        x
+                                      <:
+                                      t_Slice bool)
+                                  <:
+                                  Core.Slice.Iter.t_Iter bool)
+                              <:
+                              Core.Iter.Adapters.Enumerate.t_Enumerate (Core.Slice.Iter.t_Iter bool)
+                            )
+                            l
+                          <:
+                          Core.Iter.Adapters.Take.t_Take
+                          (Core.Iter.Adapters.Enumerate.t_Enumerate (Core.Slice.Iter.t_Iter bool)))
+                      <:
+                      Core.Iter.Adapters.Take.t_Take
+                      (Core.Iter.Adapters.Enumerate.t_Enumerate (Core.Slice.Iter.t_Iter bool)))
+                    res
+                    (fun res temp_1_ ->
+                        let res:Alloc.Vec.t_Vec Polytune.Data_types.t_Share Alloc.Alloc.t_Global =
+                          res
+                        in
+                        let l, xi:(usize & bool) = temp_1_ in
+                        let authvec:Alloc.Vec.t_Vec
+                          (Polytune.Data_types.t_Mac & Polytune.Data_types.t_Key)
+                          Alloc.Alloc.t_Global =
+                          Alloc.Vec.from_elem #(Polytune.Data_types.t_Mac &
+                              Polytune.Data_types.t_Key)
+                            ((Polytune.Data_types.Mac (mk_u128 0) <: Polytune.Data_types.t_Mac),
+                              (Polytune.Data_types.Key (mk_u128 0) <: Polytune.Data_types.t_Key)
+                              <:
+                              (Polytune.Data_types.t_Mac & Polytune.Data_types.t_Key))
+                            n
+                        in
+                        let authvec:Alloc.Vec.t_Vec
+                          (Polytune.Data_types.t_Mac & Polytune.Data_types.t_Key)
+                          Alloc.Alloc.t_Global =
+                          Rust_primitives.Hax.Folds.fold_range (mk_usize 0)
+                            n
+                            (fun authvec temp_1_ ->
+                                let authvec:Alloc.Vec.t_Vec
+                                  (Polytune.Data_types.t_Mac & Polytune.Data_types.t_Key)
+                                  Alloc.Alloc.t_Global =
+                                  authvec
+                                in
+                                let _:usize = temp_1_ in
+                                true)
+                            authvec
+                            (fun authvec k ->
+                                let authvec:Alloc.Vec.t_Vec
+                                  (Polytune.Data_types.t_Mac & Polytune.Data_types.t_Key)
+                                  Alloc.Alloc.t_Global =
+                                  authvec
+                                in
+                                let k:usize = k in
+                                if k =. i <: bool
+                                then authvec
+                                else
+                                  Rust_primitives.Hax.Monomorphized_update_at.update_at_usize authvec
+                                    k
+                                    ((Polytune.Data_types.Mac
+                                        ((macs.[ k ] <: Alloc.Vec.t_Vec u128 Alloc.Alloc.t_Global).[
+                                            l ]
+                                          <:
+                                          u128)
+                                        <:
+                                        Polytune.Data_types.t_Mac),
+                                      (Polytune.Data_types.Key
+                                        ((keys.[ k ] <: Alloc.Vec.t_Vec u128 Alloc.Alloc.t_Global).[
+                                            l ]
+                                          <:
+                                          u128)
+                                        <:
+                                        Polytune.Data_types.t_Key)
+                                      <:
+                                      (Polytune.Data_types.t_Mac & Polytune.Data_types.t_Key))
+                                  <:
+                                  Alloc.Vec.t_Vec
+                                    (Polytune.Data_types.t_Mac & Polytune.Data_types.t_Key)
+                                    Alloc.Alloc.t_Global)
+                        in
+                        Alloc.Vec.impl_1__push #Polytune.Data_types.t_Share
+                          #Alloc.Alloc.t_Global
+                          res
+                          (Polytune.Data_types.Share xi
+                              (Polytune.Data_types.Auth authvec <: Polytune.Data_types.t_Auth)
+                            <:
+                            Polytune.Data_types.t_Share))
+                in
+                let hax_temp_output:Core.Result.t_Result
+                  (Alloc.Vec.t_Vec Polytune.Data_types.t_Share Alloc.Alloc.t_Global &
+                    Rand_chacha.Chacha.t_ChaCha20Rng) t_Error =
+                  Core.Result.Result_Ok
+                  (res, multi_shared_rand
+                    <:
+                    (Alloc.Vec.t_Vec Polytune.Data_types.t_Share Alloc.Alloc.t_Global &
+                      Rand_chacha.Chacha.t_ChaCha20Rng))
                   <:
                   Core.Result.t_Result
-                    (Alloc.Vec.t_Vec (Alloc.Vec.t_Vec u128 Alloc.Alloc.t_Global)
-                        Alloc.Alloc.t_Global) t_Error
-                with
-                | Core.Result.Result_Ok di_bi_k ->
-                  let xor_xk_macs:Alloc.Vec.t_Vec (Alloc.Vec.t_Vec u128 Alloc.Alloc.t_Global)
-                    Alloc.Alloc.t_Global =
-                    Alloc.Vec.from_elem #(Alloc.Vec.t_Vec u128 Alloc.Alloc.t_Global)
-                      (Alloc.Vec.from_elem #u128 (mk_u128 0) v_RHO
-                        <:
-                        Alloc.Vec.t_Vec u128 Alloc.Alloc.t_Global)
-                      n
-                  in
-                  (match
-                      Rust_primitives.Hax.Folds.fold_range_return (mk_usize 0)
-                        v_RHO
-                        (fun xor_xk_macs temp_1_ ->
-                            let xor_xk_macs:Alloc.Vec.t_Vec
-                              (Alloc.Vec.t_Vec u128 Alloc.Alloc.t_Global) Alloc.Alloc.t_Global =
-                              xor_xk_macs
-                            in
-                            let _:usize = temp_1_ in
-                            true)
-                        xor_xk_macs
-                        (fun xor_xk_macs r ->
-                            let xor_xk_macs:Alloc.Vec.t_Vec
-                              (Alloc.Vec.t_Vec u128 Alloc.Alloc.t_Global) Alloc.Alloc.t_Global =
-                              xor_xk_macs
-                            in
-                            let r:usize = r in
-                            match
-                              Rust_primitives.Hax.Folds.fold_return (Core.Iter.Traits.Collect.f_into_iter
-                                    #(Core.Iter.Adapters.Take.t_Take
-                                      (Core.Iter.Adapters.Enumerate.t_Enumerate
-                                        (Core.Slice.Iter.t_Iter
-                                          (Alloc.Vec.t_Vec t_VectorU8 Alloc.Alloc.t_Global))))
-                                    #FStar.Tactics.Typeclasses.solve
-                                    (Core.Iter.Traits.Iterator.f_take #(Core.Iter.Adapters.Enumerate.t_Enumerate
-                                          (Core.Slice.Iter.t_Iter
-                                            (Alloc.Vec.t_Vec t_VectorU8 Alloc.Alloc.t_Global)))
-                                        #FStar.Tactics.Typeclasses.solve
-                                        (Core.Iter.Traits.Iterator.f_enumerate #(Core.Slice.Iter.t_Iter
-                                              (Alloc.Vec.t_Vec t_VectorU8 Alloc.Alloc.t_Global))
-                                            #FStar.Tactics.Typeclasses.solve
-                                            (Core.Slice.impl__iter #(Alloc.Vec.t_Vec t_VectorU8
-                                                    Alloc.Alloc.t_Global)
-                                                (Core.Ops.Deref.f_deref #(Alloc.Vec.t_Vec
-                                                        (Alloc.Vec.t_Vec t_VectorU8
-                                                            Alloc.Alloc.t_Global)
-                                                        Alloc.Alloc.t_Global)
-                                                    #FStar.Tactics.Typeclasses.solve
-                                                    dm_k
-                                                  <:
-                                                  t_Slice
-                                                  (Alloc.Vec.t_Vec t_VectorU8 Alloc.Alloc.t_Global))
-                                              <:
-                                              Core.Slice.Iter.t_Iter
-                                              (Alloc.Vec.t_Vec t_VectorU8 Alloc.Alloc.t_Global))
-                                          <:
-                                          Core.Iter.Adapters.Enumerate.t_Enumerate
-                                          (Core.Slice.Iter.t_Iter
-                                            (Alloc.Vec.t_Vec t_VectorU8 Alloc.Alloc.t_Global)))
-                                        n
-                                      <:
-                                      Core.Iter.Adapters.Take.t_Take
-                                      (Core.Iter.Adapters.Enumerate.t_Enumerate
-                                        (Core.Slice.Iter.t_Iter
-                                          (Alloc.Vec.t_Vec t_VectorU8 Alloc.Alloc.t_Global))))
-                                  <:
-                                  Core.Iter.Adapters.Take.t_Take
-                                  (Core.Iter.Adapters.Enumerate.t_Enumerate
-                                    (Core.Slice.Iter.t_Iter
-                                      (Alloc.Vec.t_Vec t_VectorU8 Alloc.Alloc.t_Global))))
-                                xor_xk_macs
-                                (fun xor_xk_macs temp_1_ ->
-                                    let xor_xk_macs:Alloc.Vec.t_Vec
-                                      (Alloc.Vec.t_Vec u128 Alloc.Alloc.t_Global)
-                                      Alloc.Alloc.t_Global =
-                                      xor_xk_macs
-                                    in
-                                    let k, dmv:(usize &
-                                      Alloc.Vec.t_Vec t_VectorU8 Alloc.Alloc.t_Global) =
-                                      temp_1_
-                                    in
-                                    match
-                                      Rust_primitives.Hax.Folds.fold_range_return (mk_usize 0)
-                                        n
-                                        (fun xor_xk_macs temp_1_ ->
-                                            let xor_xk_macs:Alloc.Vec.t_Vec
-                                              (Alloc.Vec.t_Vec u128 Alloc.Alloc.t_Global)
-                                              Alloc.Alloc.t_Global =
-                                              xor_xk_macs
-                                            in
-                                            let _:usize = temp_1_ in
-                                            true)
-                                        xor_xk_macs
-                                        (fun xor_xk_macs kk ->
-                                            let xor_xk_macs:Alloc.Vec.t_Vec
-                                              (Alloc.Vec.t_Vec u128 Alloc.Alloc.t_Global)
-                                              Alloc.Alloc.t_Global =
-                                              xor_xk_macs
-                                            in
-                                            let kk:usize = kk in
-                                            if kk =. k <: bool
-                                            then
-                                              Core.Ops.Control_flow.ControlFlow_Continue xor_xk_macs
-                                              <:
-                                              Core.Ops.Control_flow.t_ControlFlow
-                                                (Core.Ops.Control_flow.t_ControlFlow
-                                                    (iimpl_951670863_ &
-                                                      Core.Result.t_Result
-                                                        (Alloc.Vec.t_Vec Polytune.Data_types.t_Share
-                                                            Alloc.Alloc.t_Global &
-                                                          Rand_chacha.Chacha.t_ChaCha20Rng) t_Error)
-                                                    (Prims.unit &
-                                                      Alloc.Vec.t_Vec
-                                                        (Alloc.Vec.t_Vec u128 Alloc.Alloc.t_Global)
-                                                        Alloc.Alloc.t_Global))
-                                                (Alloc.Vec.t_Vec
-                                                    (Alloc.Vec.t_Vec u128 Alloc.Alloc.t_Global)
-                                                    Alloc.Alloc.t_Global)
-                                            else
-                                              if
-                                                Alloc.Vec.impl_1__is_empty #t_VectorU8
-                                                  #Alloc.Alloc.t_Global
-                                                  dmv
-                                                <:
-                                                bool
-                                              then
-                                                Core.Ops.Control_flow.ControlFlow_Break
-                                                (Core.Ops.Control_flow.ControlFlow_Break
-                                                  (channel,
-                                                    (Core.Result.Result_Err
-                                                      (Error_EmptyVector <: t_Error)
-                                                      <:
-                                                      Core.Result.t_Result
-                                                        (Alloc.Vec.t_Vec Polytune.Data_types.t_Share
-                                                            Alloc.Alloc.t_Global &
-                                                          Rand_chacha.Chacha.t_ChaCha20Rng) t_Error)
-                                                    <:
-                                                    (iimpl_951670863_ &
-                                                      Core.Result.t_Result
-                                                        (Alloc.Vec.t_Vec Polytune.Data_types.t_Share
-                                                            Alloc.Alloc.t_Global &
-                                                          Rand_chacha.Chacha.t_ChaCha20Rng) t_Error)
-                                                  )
-                                                  <:
-                                                  Core.Ops.Control_flow.t_ControlFlow
-                                                    (iimpl_951670863_ &
-                                                      Core.Result.t_Result
-                                                        (Alloc.Vec.t_Vec Polytune.Data_types.t_Share
-                                                            Alloc.Alloc.t_Global &
-                                                          Rand_chacha.Chacha.t_ChaCha20Rng) t_Error)
-                                                    (Prims.unit &
-                                                      Alloc.Vec.t_Vec
-                                                        (Alloc.Vec.t_Vec u128 Alloc.Alloc.t_Global)
-                                                        Alloc.Alloc.t_Global))
-                                                <:
-                                                Core.Ops.Control_flow.t_ControlFlow
-                                                  (Core.Ops.Control_flow.t_ControlFlow
-                                                      (iimpl_951670863_ &
-                                                        Core.Result.t_Result
-                                                          (Alloc.Vec.t_Vec
-                                                              Polytune.Data_types.t_Share
-                                                              Alloc.Alloc.t_Global &
-                                                            Rand_chacha.Chacha.t_ChaCha20Rng)
-                                                          t_Error)
-                                                      (Prims.unit &
-                                                        Alloc.Vec.t_Vec
-                                                          (Alloc.Vec.t_Vec u128 Alloc.Alloc.t_Global
-                                                          ) Alloc.Alloc.t_Global))
-                                                  (Alloc.Vec.t_Vec
-                                                      (Alloc.Vec.t_Vec u128 Alloc.Alloc.t_Global)
-                                                      Alloc.Alloc.t_Global)
-                                              else
-                                                let dm:t_VectorU8 = dmv.[ r ] in
-                                                let start:usize =
-                                                  if kk >. k
-                                                  then
-                                                    mk_usize 1 +!
-                                                    ((kk -! mk_usize 1 <: usize) *! mk_usize 16
-                                                      <:
-                                                      usize)
-                                                  else mk_usize 1 +! (kk *! mk_usize 16 <: usize)
-                                                in
-                                                let v_end:usize = start +! mk_usize 16 in
-                                                match
-                                                  Core.Result.impl__map #(t_Array u8 (mk_usize 16))
-                                                    #Core.Array.t_TryFromSliceError
-                                                    #u128
-                                                    (Core.Convert.f_try_into #(t_Slice u8)
-                                                        #(t_Array u8 (mk_usize 16))
-                                                        #FStar.Tactics.Typeclasses.solve
-                                                        (dm._0.[ {
-                                                              Core.Ops.Range.f_start = start;
-                                                              Core.Ops.Range.f_end = v_end
-                                                            }
-                                                            <:
-                                                            Core.Ops.Range.t_Range usize ]
-                                                          <:
-                                                          t_Slice u8)
-                                                      <:
-                                                      Core.Result.t_Result
-                                                        (t_Array u8 (mk_usize 16))
-                                                        Core.Array.t_TryFromSliceError)
-                                                    Core.Num.impl_u128__from_be_bytes
-                                                  <:
-                                                  Core.Result.t_Result u128
-                                                    Core.Array.t_TryFromSliceError
-                                                with
-                                                | Core.Result.Result_Ok mac ->
-                                                  let xor_xk_macs:Alloc.Vec.t_Vec
-                                                    (Alloc.Vec.t_Vec u128 Alloc.Alloc.t_Global)
-                                                    Alloc.Alloc.t_Global =
-                                                    Rust_primitives.Hax.Monomorphized_update_at.update_at_usize
-                                                      xor_xk_macs
-                                                      kk
-                                                      (Rust_primitives.Hax.Monomorphized_update_at.update_at_usize
-                                                          (xor_xk_macs.[ kk ]
-                                                            <:
-                                                            Alloc.Vec.t_Vec u128
-                                                              Alloc.Alloc.t_Global)
-                                                          r
-                                                          (mac ^.
-                                                            ((xor_xk_macs.[ kk ]
-                                                                <:
-                                                                Alloc.Vec.t_Vec u128
-                                                                  Alloc.Alloc.t_Global).[ r ]
-                                                              <:
-                                                              u128)
-                                                            <:
-                                                            u128)
-                                                        <:
-                                                        Alloc.Vec.t_Vec u128 Alloc.Alloc.t_Global)
-                                                  in
-                                                  Core.Ops.Control_flow.ControlFlow_Continue
-                                                  xor_xk_macs
-                                                  <:
-                                                  Core.Ops.Control_flow.t_ControlFlow
-                                                    (Core.Ops.Control_flow.t_ControlFlow
-                                                        (iimpl_951670863_ &
-                                                          Core.Result.t_Result
-                                                            (Alloc.Vec.t_Vec
-                                                                Polytune.Data_types.t_Share
-                                                                Alloc.Alloc.t_Global &
-                                                              Rand_chacha.Chacha.t_ChaCha20Rng)
-                                                            t_Error)
-                                                        (Prims.unit &
-                                                          Alloc.Vec.t_Vec
-                                                            (Alloc.Vec.t_Vec u128
-                                                                Alloc.Alloc.t_Global)
-                                                            Alloc.Alloc.t_Global))
-                                                    (Alloc.Vec.t_Vec
-                                                        (Alloc.Vec.t_Vec u128 Alloc.Alloc.t_Global)
-                                                        Alloc.Alloc.t_Global)
-                                                | _ ->
-                                                  Core.Ops.Control_flow.ControlFlow_Break
-                                                  (Core.Ops.Control_flow.ControlFlow_Break
-                                                    (channel,
-                                                      (Core.Result.Result_Err
-                                                        (Error_ConversionErr <: t_Error)
-                                                        <:
-                                                        Core.Result.t_Result
-                                                          (Alloc.Vec.t_Vec
-                                                              Polytune.Data_types.t_Share
-                                                              Alloc.Alloc.t_Global &
-                                                            Rand_chacha.Chacha.t_ChaCha20Rng)
-                                                          t_Error)
-                                                      <:
-                                                      (iimpl_951670863_ &
-                                                        Core.Result.t_Result
-                                                          (Alloc.Vec.t_Vec
-                                                              Polytune.Data_types.t_Share
-                                                              Alloc.Alloc.t_Global &
-                                                            Rand_chacha.Chacha.t_ChaCha20Rng)
-                                                          t_Error))
-                                                    <:
-                                                    Core.Ops.Control_flow.t_ControlFlow
-                                                      (iimpl_951670863_ &
-                                                        Core.Result.t_Result
-                                                          (Alloc.Vec.t_Vec
-                                                              Polytune.Data_types.t_Share
-                                                              Alloc.Alloc.t_Global &
-                                                            Rand_chacha.Chacha.t_ChaCha20Rng)
-                                                          t_Error)
-                                                      (Prims.unit &
-                                                        Alloc.Vec.t_Vec
-                                                          (Alloc.Vec.t_Vec u128 Alloc.Alloc.t_Global
-                                                          ) Alloc.Alloc.t_Global))
-                                                  <:
-                                                  Core.Ops.Control_flow.t_ControlFlow
-                                                    (Core.Ops.Control_flow.t_ControlFlow
-                                                        (iimpl_951670863_ &
-                                                          Core.Result.t_Result
-                                                            (Alloc.Vec.t_Vec
-                                                                Polytune.Data_types.t_Share
-                                                                Alloc.Alloc.t_Global &
-                                                              Rand_chacha.Chacha.t_ChaCha20Rng)
-                                                            t_Error)
-                                                        (Prims.unit &
-                                                          Alloc.Vec.t_Vec
-                                                            (Alloc.Vec.t_Vec u128
-                                                                Alloc.Alloc.t_Global)
-                                                            Alloc.Alloc.t_Global))
-                                                    (Alloc.Vec.t_Vec
-                                                        (Alloc.Vec.t_Vec u128 Alloc.Alloc.t_Global)
-                                                        Alloc.Alloc.t_Global))
-                                      <:
-                                      Core.Ops.Control_flow.t_ControlFlow
-                                        (iimpl_951670863_ &
-                                          Core.Result.t_Result
-                                            (Alloc.Vec.t_Vec Polytune.Data_types.t_Share
-                                                Alloc.Alloc.t_Global &
-                                              Rand_chacha.Chacha.t_ChaCha20Rng) t_Error)
-                                        (Alloc.Vec.t_Vec (Alloc.Vec.t_Vec u128 Alloc.Alloc.t_Global)
-                                            Alloc.Alloc.t_Global)
-                                    with
-                                    | Core.Ops.Control_flow.ControlFlow_Break ret ->
-                                      Core.Ops.Control_flow.ControlFlow_Break
-                                      (Core.Ops.Control_flow.ControlFlow_Break ret
-                                        <:
-                                        Core.Ops.Control_flow.t_ControlFlow
-                                          (iimpl_951670863_ &
-                                            Core.Result.t_Result
-                                              (Alloc.Vec.t_Vec Polytune.Data_types.t_Share
-                                                  Alloc.Alloc.t_Global &
-                                                Rand_chacha.Chacha.t_ChaCha20Rng) t_Error)
-                                          (Prims.unit &
-                                            Alloc.Vec.t_Vec
-                                              (Alloc.Vec.t_Vec u128 Alloc.Alloc.t_Global)
-                                              Alloc.Alloc.t_Global))
-                                      <:
-                                      Core.Ops.Control_flow.t_ControlFlow
-                                        (Core.Ops.Control_flow.t_ControlFlow
-                                            (iimpl_951670863_ &
-                                              Core.Result.t_Result
-                                                (Alloc.Vec.t_Vec Polytune.Data_types.t_Share
-                                                    Alloc.Alloc.t_Global &
-                                                  Rand_chacha.Chacha.t_ChaCha20Rng) t_Error)
-                                            (Prims.unit &
-                                              Alloc.Vec.t_Vec
-                                                (Alloc.Vec.t_Vec u128 Alloc.Alloc.t_Global)
-                                                Alloc.Alloc.t_Global))
-                                        (Alloc.Vec.t_Vec (Alloc.Vec.t_Vec u128 Alloc.Alloc.t_Global)
-                                            Alloc.Alloc.t_Global)
-                                    | Core.Ops.Control_flow.ControlFlow_Continue loop_res ->
-                                      Core.Ops.Control_flow.ControlFlow_Continue loop_res
-                                      <:
-                                      Core.Ops.Control_flow.t_ControlFlow
-                                        (Core.Ops.Control_flow.t_ControlFlow
-                                            (iimpl_951670863_ &
-                                              Core.Result.t_Result
-                                                (Alloc.Vec.t_Vec Polytune.Data_types.t_Share
-                                                    Alloc.Alloc.t_Global &
-                                                  Rand_chacha.Chacha.t_ChaCha20Rng) t_Error)
-                                            (Prims.unit &
-                                              Alloc.Vec.t_Vec
-                                                (Alloc.Vec.t_Vec u128 Alloc.Alloc.t_Global)
-                                                Alloc.Alloc.t_Global))
-                                        (Alloc.Vec.t_Vec (Alloc.Vec.t_Vec u128 Alloc.Alloc.t_Global)
-                                            Alloc.Alloc.t_Global))
-                              <:
-                              Core.Ops.Control_flow.t_ControlFlow
-                                (iimpl_951670863_ &
-                                  Core.Result.t_Result
-                                    (Alloc.Vec.t_Vec Polytune.Data_types.t_Share
-                                        Alloc.Alloc.t_Global &
-                                      Rand_chacha.Chacha.t_ChaCha20Rng) t_Error)
-                                (Alloc.Vec.t_Vec (Alloc.Vec.t_Vec u128 Alloc.Alloc.t_Global)
-                                    Alloc.Alloc.t_Global)
-                            with
-                            | Core.Ops.Control_flow.ControlFlow_Break ret ->
-                              Core.Ops.Control_flow.ControlFlow_Break
-                              (Core.Ops.Control_flow.ControlFlow_Break ret
-                                <:
-                                Core.Ops.Control_flow.t_ControlFlow
-                                  (iimpl_951670863_ &
-                                    Core.Result.t_Result
-                                      (Alloc.Vec.t_Vec Polytune.Data_types.t_Share
-                                          Alloc.Alloc.t_Global &
-                                        Rand_chacha.Chacha.t_ChaCha20Rng) t_Error)
-                                  (Prims.unit &
-                                    Alloc.Vec.t_Vec (Alloc.Vec.t_Vec u128 Alloc.Alloc.t_Global)
-                                      Alloc.Alloc.t_Global))
-                              <:
-                              Core.Ops.Control_flow.t_ControlFlow
-                                (Core.Ops.Control_flow.t_ControlFlow
-                                    (iimpl_951670863_ &
-                                      Core.Result.t_Result
-                                        (Alloc.Vec.t_Vec Polytune.Data_types.t_Share
-                                            Alloc.Alloc.t_Global &
-                                          Rand_chacha.Chacha.t_ChaCha20Rng) t_Error)
-                                    (Prims.unit &
-                                      Alloc.Vec.t_Vec (Alloc.Vec.t_Vec u128 Alloc.Alloc.t_Global)
-                                        Alloc.Alloc.t_Global))
-                                (Alloc.Vec.t_Vec (Alloc.Vec.t_Vec u128 Alloc.Alloc.t_Global)
-                                    Alloc.Alloc.t_Global)
-                            | Core.Ops.Control_flow.ControlFlow_Continue xor_xk_macs ->
-                              match
-                                Rust_primitives.Hax.Folds.fold_range_return (mk_usize 0)
-                                  n
-                                  (fun temp_0_ temp_1_ ->
-                                      let _:Prims.unit = temp_0_ in
-                                      let _:usize = temp_1_ in
-                                      true)
-                                  ()
-                                  (fun temp_0_ k ->
-                                      let _:Prims.unit = temp_0_ in
-                                      let k:usize = k in
-                                      if k =. i <: bool
-                                      then
-                                        Core.Ops.Control_flow.ControlFlow_Continue
-                                        (() <: Prims.unit)
-                                        <:
-                                        Core.Ops.Control_flow.t_ControlFlow
-                                          (Core.Ops.Control_flow.t_ControlFlow
-                                              (iimpl_951670863_ &
-                                                Core.Result.t_Result
-                                                  (Alloc.Vec.t_Vec Polytune.Data_types.t_Share
-                                                      Alloc.Alloc.t_Global &
-                                                    Rand_chacha.Chacha.t_ChaCha20Rng) t_Error)
-                                              (Prims.unit & Prims.unit)) Prims.unit
-                                      else
-                                        let d_bj:t_Array u8 (mk_usize 16) =
-                                          Core.Num.impl_u128__to_be_bytes ((di_bi_k.[ k ]
-                                                <:
-                                                Alloc.Vec.t_Vec u128 Alloc.Alloc.t_Global).[ r ]
-                                              <:
-                                              u128)
-                                        in
-                                        let commitments:t_CommitmentTriple =
-                                          (c0_c1_cm_k.[ k ]
-                                            <:
-                                            Alloc.Vec.t_Vec t_CommitmentTriple Alloc.Alloc.t_Global).[
-                                            r ]
-                                        in
-                                        if
-                                          ~.(open_commitment commitments._0 (d_bj <: t_Slice u8)
-                                            <:
-                                            bool) &&
-                                          ~.(open_commitment commitments._1 (d_bj <: t_Slice u8)
-                                            <:
-                                            bool)
-                                        then
-                                          Core.Ops.Control_flow.ControlFlow_Break
-                                          (Core.Ops.Control_flow.ControlFlow_Break
-                                            (channel,
-                                              (Core.Result.Result_Err
-                                                (Error_CommitmentCouldNotBeOpened <: t_Error)
-                                                <:
-                                                Core.Result.t_Result
-                                                  (Alloc.Vec.t_Vec Polytune.Data_types.t_Share
-                                                      Alloc.Alloc.t_Global &
-                                                    Rand_chacha.Chacha.t_ChaCha20Rng) t_Error)
-                                              <:
-                                              (iimpl_951670863_ &
-                                                Core.Result.t_Result
-                                                  (Alloc.Vec.t_Vec Polytune.Data_types.t_Share
-                                                      Alloc.Alloc.t_Global &
-                                                    Rand_chacha.Chacha.t_ChaCha20Rng) t_Error))
-                                            <:
-                                            Core.Ops.Control_flow.t_ControlFlow
-                                              (iimpl_951670863_ &
-                                                Core.Result.t_Result
-                                                  (Alloc.Vec.t_Vec Polytune.Data_types.t_Share
-                                                      Alloc.Alloc.t_Global &
-                                                    Rand_chacha.Chacha.t_ChaCha20Rng) t_Error)
-                                              (Prims.unit & Prims.unit))
-                                          <:
-                                          Core.Ops.Control_flow.t_ControlFlow
-                                            (Core.Ops.Control_flow.t_ControlFlow
-                                                (iimpl_951670863_ &
-                                                  Core.Result.t_Result
-                                                    (Alloc.Vec.t_Vec Polytune.Data_types.t_Share
-                                                        Alloc.Alloc.t_Global &
-                                                      Rand_chacha.Chacha.t_ChaCha20Rng) t_Error)
-                                                (Prims.unit & Prims.unit)) Prims.unit
-                                        else
-                                          if
-                                            ((xor_xk_macs.[ k ]
-                                                <:
-                                                Alloc.Vec.t_Vec u128 Alloc.Alloc.t_Global).[ r ]
-                                              <:
-                                              u128) <>.
-                                            ((di_bi_k.[ k ]
-                                                <:
-                                                Alloc.Vec.t_Vec u128 Alloc.Alloc.t_Global).[ r ]
-                                              <:
-                                              u128)
-                                          then
-                                            Core.Ops.Control_flow.ControlFlow_Break
-                                            (Core.Ops.Control_flow.ControlFlow_Break
-                                              (channel,
-                                                (Core.Result.Result_Err
-                                                  (Error_AShareWrongMAC <: t_Error)
-                                                  <:
-                                                  Core.Result.t_Result
-                                                    (Alloc.Vec.t_Vec Polytune.Data_types.t_Share
-                                                        Alloc.Alloc.t_Global &
-                                                      Rand_chacha.Chacha.t_ChaCha20Rng) t_Error)
-                                                <:
-                                                (iimpl_951670863_ &
-                                                  Core.Result.t_Result
-                                                    (Alloc.Vec.t_Vec Polytune.Data_types.t_Share
-                                                        Alloc.Alloc.t_Global &
-                                                      Rand_chacha.Chacha.t_ChaCha20Rng) t_Error))
-                                              <:
-                                              Core.Ops.Control_flow.t_ControlFlow
-                                                (iimpl_951670863_ &
-                                                  Core.Result.t_Result
-                                                    (Alloc.Vec.t_Vec Polytune.Data_types.t_Share
-                                                        Alloc.Alloc.t_Global &
-                                                      Rand_chacha.Chacha.t_ChaCha20Rng) t_Error)
-                                                (Prims.unit & Prims.unit))
-                                            <:
-                                            Core.Ops.Control_flow.t_ControlFlow
-                                              (Core.Ops.Control_flow.t_ControlFlow
-                                                  (iimpl_951670863_ &
-                                                    Core.Result.t_Result
-                                                      (Alloc.Vec.t_Vec Polytune.Data_types.t_Share
-                                                          Alloc.Alloc.t_Global &
-                                                        Rand_chacha.Chacha.t_ChaCha20Rng) t_Error)
-                                                  (Prims.unit & Prims.unit)) Prims.unit
-                                          else
-                                            Core.Ops.Control_flow.ControlFlow_Continue ()
-                                            <:
-                                            Core.Ops.Control_flow.t_ControlFlow
-                                              (Core.Ops.Control_flow.t_ControlFlow
-                                                  (iimpl_951670863_ &
-                                                    Core.Result.t_Result
-                                                      (Alloc.Vec.t_Vec Polytune.Data_types.t_Share
-                                                          Alloc.Alloc.t_Global &
-                                                        Rand_chacha.Chacha.t_ChaCha20Rng) t_Error)
-                                                  (Prims.unit & Prims.unit)) Prims.unit)
-                                <:
-                                Core.Ops.Control_flow.t_ControlFlow
-                                  (iimpl_951670863_ &
-                                    Core.Result.t_Result
-                                      (Alloc.Vec.t_Vec Polytune.Data_types.t_Share
-                                          Alloc.Alloc.t_Global &
-                                        Rand_chacha.Chacha.t_ChaCha20Rng) t_Error) Prims.unit
-                              with
-                              | Core.Ops.Control_flow.ControlFlow_Break ret ->
-                                Core.Ops.Control_flow.ControlFlow_Break
-                                (Core.Ops.Control_flow.ControlFlow_Break ret
-                                  <:
-                                  Core.Ops.Control_flow.t_ControlFlow
-                                    (iimpl_951670863_ &
-                                      Core.Result.t_Result
-                                        (Alloc.Vec.t_Vec Polytune.Data_types.t_Share
-                                            Alloc.Alloc.t_Global &
-                                          Rand_chacha.Chacha.t_ChaCha20Rng) t_Error)
-                                    (Prims.unit &
-                                      Alloc.Vec.t_Vec (Alloc.Vec.t_Vec u128 Alloc.Alloc.t_Global)
-                                        Alloc.Alloc.t_Global))
-                                <:
-                                Core.Ops.Control_flow.t_ControlFlow
-                                  (Core.Ops.Control_flow.t_ControlFlow
-                                      (iimpl_951670863_ &
-                                        Core.Result.t_Result
-                                          (Alloc.Vec.t_Vec Polytune.Data_types.t_Share
-                                              Alloc.Alloc.t_Global &
-                                            Rand_chacha.Chacha.t_ChaCha20Rng) t_Error)
-                                      (Prims.unit &
-                                        Alloc.Vec.t_Vec (Alloc.Vec.t_Vec u128 Alloc.Alloc.t_Global)
-                                          Alloc.Alloc.t_Global))
-                                  (Alloc.Vec.t_Vec (Alloc.Vec.t_Vec u128 Alloc.Alloc.t_Global)
-                                      Alloc.Alloc.t_Global)
-                              | Core.Ops.Control_flow.ControlFlow_Continue () ->
-                                Core.Ops.Control_flow.ControlFlow_Continue xor_xk_macs
-                                <:
-                                Core.Ops.Control_flow.t_ControlFlow
-                                  (Core.Ops.Control_flow.t_ControlFlow
-                                      (iimpl_951670863_ &
-                                        Core.Result.t_Result
-                                          (Alloc.Vec.t_Vec Polytune.Data_types.t_Share
-                                              Alloc.Alloc.t_Global &
-                                            Rand_chacha.Chacha.t_ChaCha20Rng) t_Error)
-                                      (Prims.unit &
-                                        Alloc.Vec.t_Vec (Alloc.Vec.t_Vec u128 Alloc.Alloc.t_Global)
-                                          Alloc.Alloc.t_Global))
-                                  (Alloc.Vec.t_Vec (Alloc.Vec.t_Vec u128 Alloc.Alloc.t_Global)
-                                      Alloc.Alloc.t_Global))
-                      <:
-                      Core.Ops.Control_flow.t_ControlFlow
-                        (iimpl_951670863_ &
-                          Core.Result.t_Result
-                            (Alloc.Vec.t_Vec Polytune.Data_types.t_Share Alloc.Alloc.t_Global &
-                              Rand_chacha.Chacha.t_ChaCha20Rng) t_Error)
-                        (Alloc.Vec.t_Vec (Alloc.Vec.t_Vec u128 Alloc.Alloc.t_Global)
-                            Alloc.Alloc.t_Global)
-                    with
-                    | Core.Ops.Control_flow.ControlFlow_Break ret -> ret
-                    | Core.Ops.Control_flow.ControlFlow_Continue xor_xk_macs ->
-                      let xishares:Alloc.Vec.t_Vec Polytune.Data_types.t_Share Alloc.Alloc.t_Global
-                      =
-                        Alloc.Vec.impl_1__truncate #Polytune.Data_types.t_Share
-                          #Alloc.Alloc.t_Global
-                          xishares
-                          l
-                      in
-                      let hax_temp_output:Core.Result.t_Result
-                        (Alloc.Vec.t_Vec Polytune.Data_types.t_Share Alloc.Alloc.t_Global &
-                          Rand_chacha.Chacha.t_ChaCha20Rng) t_Error =
-                        Core.Result.Result_Ok
-                        (xishares, multi_shared_rand
-                          <:
-                          (Alloc.Vec.t_Vec Polytune.Data_types.t_Share Alloc.Alloc.t_Global &
-                            Rand_chacha.Chacha.t_ChaCha20Rng))
-                        <:
-                        Core.Result.t_Result
-                          (Alloc.Vec.t_Vec Polytune.Data_types.t_Share Alloc.Alloc.t_Global &
-                            Rand_chacha.Chacha.t_ChaCha20Rng) t_Error
-                      in
-                      channel, hax_temp_output
-                      <:
-                      (iimpl_951670863_ &
-                        Core.Result.t_Result
-                          (Alloc.Vec.t_Vec Polytune.Data_types.t_Share Alloc.Alloc.t_Global &
-                            Rand_chacha.Chacha.t_ChaCha20Rng) t_Error))
-                | Core.Result.Result_Err err ->
-                  channel,
-                  (Core.Result.Result_Err err
-                    <:
-                    Core.Result.t_Result
-                      (Alloc.Vec.t_Vec Polytune.Data_types.t_Share Alloc.Alloc.t_Global &
-                        Rand_chacha.Chacha.t_ChaCha20Rng) t_Error)
-                  <:
-                  (iimpl_951670863_ &
-                    Core.Result.t_Result
-                      (Alloc.Vec.t_Vec Polytune.Data_types.t_Share Alloc.Alloc.t_Global &
-                        Rand_chacha.Chacha.t_ChaCha20Rng) t_Error))
+                    (Alloc.Vec.t_Vec Polytune.Data_types.t_Share Alloc.Alloc.t_Global &
+                      Rand_chacha.Chacha.t_ChaCha20Rng) t_Error
+                in
+                channel, hax_temp_output
+                <:
+                (iimpl_951670863_ &
+                  Core.Result.t_Result
+                    (Alloc.Vec.t_Vec Polytune.Data_types.t_Share Alloc.Alloc.t_Global &
+                      Rand_chacha.Chacha.t_ChaCha20Rng) t_Error))
           | Core.Result.Result_Err err ->
             channel,
             (Core.Result.Result_Err err
@@ -1339,16 +1301,4 @@ let fashare
         (iimpl_951670863_ &
           Core.Result.t_Result
             (Alloc.Vec.t_Vec Polytune.Data_types.t_Share Alloc.Alloc.t_Global &
-              Rand_chacha.Chacha.t_ChaCha20Rng) t_Error))
-  | Core.Result.Result_Err err ->
-    channel,
-    (Core.Result.Result_Err err
-      <:
-      Core.Result.t_Result
-        (Alloc.Vec.t_Vec Polytune.Data_types.t_Share Alloc.Alloc.t_Global &
-          Rand_chacha.Chacha.t_ChaCha20Rng) t_Error)
-    <:
-    (iimpl_951670863_ &
-      Core.Result.t_Result
-        (Alloc.Vec.t_Vec Polytune.Data_types.t_Share Alloc.Alloc.t_Global &
-          Rand_chacha.Chacha.t_ChaCha20Rng) t_Error)
+              Rand_chacha.Chacha.t_ChaCha20Rng) t_Error)
