proofs/fstar/extraction/Rand.Rng.fst
@@ -1,0 +1,6 @@
+module Rand.Rng
+#set-options "--fuel 0 --ifuel 1 --z3rlimit 15"
+
+class t_Rng (t_Self:Type) = {
+  f_gen: t_Self -> t_Self
+}
