proofs/fstar/extraction/Rand.fst
@@ -1,0 +1,6 @@
+module Rand
+#set-options "--fuel 0 --ifuel 1 --z3rlimit 15"
+
+class t_Rand (t_Self:Type) = {
+  random: unit -> t_Self
+}
